Only exponential left

AsynchronousGames.v
@@ -1,5 +1,6 @@
 Require Import List.
 Require Import ZArith.
+Require Import Group.
 
 Record PartialOrder :=
   {
@@ -78,8 +79,9 @@ Record AsynchronousArena := {
     finite_payoff_walk : Walk E -> Z;
     infinite_payoff : InfinitePosition E  -> Infinity;
 
-    initial_payoff :
-    finite_payoff_position nil = (-1)%Z \/ finite_payoff_position nil = (1)%Z;
+    initial_payoff : sumbool
+    (finite_payoff_position nil = (-1)%Z)
+    (finite_payoff_position nil = (1)%Z);
 
     polarity_first : forall m, initial_move (P E) m -> 
     ((polarity m = true -> finite_payoff_position nil = (-1)%Z)
@@ -100,20 +102,6 @@ Record AsynchronousArena := {
     (fst (fst w)) = nil) -> 
     finite_payoff_walk w = 
     finite_payoff_position ((fst (snd w)) ++ (snd (snd w)));*)
-}.
-
-Record Group := {
-      G : Type;
-      mult : G -> G -> G;
-      id : G;
-      inverse : G -> G;
-
-      associative : forall (x y z : G),
-      mult x (mult y z) = mult (mult x y) z;
-      id_exists : forall (x : G), 
-      mult id x = x /\ mult x id = x;
-      inverses_exist : forall (x : G),
-      mult x (inverse x) = id /\ mult (inverse x) x = id;
 }.
 
 Record AsynchronousGame  := 
@@ -149,90 +137,7 @@ Record AsynchronousGame  :=
     exists i' m', action g (existT _ i (inr m)) h = existT _ i' (inr m');
 }.
 
-Fact inverse_is_unique (G: Group) : forall x y z,
-mult G x y = id G /\ mult G x z = id G -> y = z.
-Proof. intros. destruct H. rewrite <- H in H0.
-assert (mult G (inverse G x) (mult G x z) = 
-mult G (inverse G x) (mult G x y) ).
-{  rewrite H0. reflexivity. }
-rewrite associative in H1. rewrite associative in H1.
-assert (mult G (inverse G x) x = id G).
-{ apply inverses_exist. }
-rewrite H2 in H1. 
-assert (mult G (id G) z = z /\ mult G (id G) y = y).
-{ split. 
-+ apply id_exists.
-+ apply id_exists. }
-destruct H3. rewrite H3 in H1. rewrite H4 in H1. auto.
-Qed.
 
-Fact mult_inverse (G: Group) : forall g g',
-mult G (inverse G g') (inverse G g) = inverse G (mult G g g').
-Proof. intros. 
-assert (mult G (mult G g g') (mult G (inverse G g') (inverse G g)) = id G /\
-mult G (mult G g g') (inverse G (mult G g g')) = id G).
-{ assert (mult G (mult G g g') (inverse G (mult G g g')) = id G).
-{ apply inverses_exist. }
-assert (mult G (mult G g g') (mult G (inverse G g') (inverse G g)) = id G).
-{ rewrite associative. 
-assert (mult G (mult G g g') (inverse G g') = g).
-{ rewrite <- associative.
-assert (mult G g' (inverse G g') = id G).
-{ apply inverses_exist. }
-rewrite H0. apply id_exists.
-  }
-rewrite H0. apply inverses_exist.
- }
-rewrite H. rewrite H0. auto.
-} apply inverse_is_unique with (G0:=G) (x:=mult G g g')
-(y:=mult G (inverse G g') (inverse G g)) (z:=inverse G (mult G g g')).
-auto.
-Qed.
-
-Fact inverse_id_is_id (G: Group) : inverse G (id G) = id G.
-Proof. apply inverse_is_unique with (G0:=G) (x:=id G) 
-(y:= inverse G (id G)) (z:=id G). 
-split.
-+ apply inverses_exist.
-+ apply id_exists.
-Qed.
-
-Definition trivial_group : Group.
-refine({|
-          G := unit;
-          mult a b := tt;
-          id := tt
-      |}).
-Proof.
-- auto.
-- auto.
-- intros. destruct x. auto.
-- auto.
-Defined.
-
-Definition product_group (X Y : Group) : Group.
-refine ({|
-        G := (G X) * (G Y);
-        mult m n := (mult _ (fst m) (fst n), mult _ (snd m) (snd n));
-        id := (id _, id _);
-        inverse m := (inverse _ (fst m), inverse _ (snd m))
-       |}).
-Proof.
-- intros. destruct x. destruct y. destruct z. simpl.
-rewrite associative. rewrite associative. reflexivity.
-- intros. destruct x. simpl.
-assert (mult _ (id _) g = g /\ mult _ g (id _) = g).
-{ apply id_exists. }
-assert (mult _ (id _) g0 = g0 /\ mult _ g0 (id _) = g0).
-{ apply id_exists. }
-destruct H0. destruct H. rewrite H. rewrite H1. rewrite H0. rewrite H2. auto.
-- intros. destruct x. simpl. 
-assert (mult _ g (inverse _ g) = id _ /\ mult _ (inverse _ g) g = id _).
-{ apply inverses_exist. }
-assert (mult _ g0 (inverse _ g0) = id _ /\ mult _ (inverse _ g0) g0 = id _).
-{ apply inverses_exist. }
-destruct H. destruct H0. rewrite H. rewrite H1. rewrite H0. rewrite H2. auto.
-Defined.
 
 Definition valid_position (E : EventStructure) (p : Position E) :=
 forall m n, (In n p -> leq (P E) m n -> In m p)
@@ -254,5 +159,17 @@ valid_path E (fst w) /\ valid_path E (snd w) /\
 (forall x,  In x (fst (fst w)) <-> In x (fst (snd w))).
 
 
+Ltac flatten_all :=
+  repeat (let e := fresh "e" in
+      match goal with
+      | h: context[match ?x with | _ => _ end] |- _ => destruct x eqn:e
+      | |- context[match ?x with | _ => _ end] => destruct x eqn:e
+      end).
 
+Ltac flatten :=
+  repeat (let e := fresh "e" in
+      match goal with
+      | h: context[match ?x with | _ => _ end] |- _ => destruct x eqn:e
+      | |- context[match ?x with | _ => _ end] => destruct x eqn:e
+      end).
 
