Dual.v
@@ -1,0 +1,89 @@
+Require Import List.
+Require Import ZArith.
+Require Import Lia.
+Require Import Init.Nat.
+Require Import Logic.Eqdep.
+Require Import Logic.Eqdep_dec.
+Require Import Arith.PeanoNat.
+Require Import Bool.Bool.
+Require Import AsynchronousGames.
+
+Fixpoint neg_inf i :=
+match i with
+| plus_infinity => minus_infinity
+| minus_infinity => plus_infinity
+end.
+
+Definition asynchronous_arena_dual (A: AsynchronousArena) 
+: AsynchronousArena.
+  refine({| 
+            E := E A ;
+            polarity m := negb (polarity A m);
+            finite_payoff_position l := Z.sub 0 (finite_payoff_position A l);
+            finite_payoff_walk w := Z.sub 0 (finite_payoff_walk A w);
+            infinite_payoff l := neg_inf (infinite_payoff A l);
+         |}).
+Proof.
+- intros. simpl. 
+assert ((finite_payoff_position A nil = (-1)%Z) +
+    (finite_payoff_position A nil = (1)%Z)).
+{destruct (initial_payoff A).
++ left. auto.
++ right. auto. }
+assert ((- finite_payoff_position A nil)%Z = (-1)%Z <->
+(finite_payoff_position A nil)%Z = (1)%Z).
+{lia. }
+assert ((- finite_payoff_position A nil)%Z = 1%Z <->
+(finite_payoff_position A nil)%Z = (-1)%Z).
+{lia. } destruct H.
++ rewrite <- H1 in e. right. auto.
++ rewrite <- H0 in e. left. auto.
+- intros. simpl. split.
++ intros. apply negb_true_iff in H0. apply polarity_first in H.
+apply H in H0.
+assert ((- finite_payoff_position A nil)%Z = (-1)%Z <->
+(finite_payoff_position A nil)%Z = (1)%Z).
+{lia. } apply H1. auto.
++ intros. apply negb_false_iff in H0. apply polarity_first in H.
+apply H in H0.
+assert ((- finite_payoff_position A nil)%Z = 1%Z <->
+(finite_payoff_position A nil)%Z = (-1)%Z).
+{lia. } apply H1. auto.
+- intros. apply polarity_second in H. split.
++ intros. apply negb_true_iff in H0. apply H in H0. simpl.
+assert ((- finite_payoff_position A nil)%Z = 1%Z <->
+(finite_payoff_position A nil)%Z = (-1)%Z).
+{lia. } rewrite H1. auto.
++ intros. apply negb_false_iff in H0. apply H in H0. simpl.
+assert ((- finite_payoff_position A nil)%Z = (-1)%Z <->
+(finite_payoff_position A nil)%Z = (1)%Z).
+{lia. } apply H1. auto.
+- intros. simpl.
+assert ((- finite_payoff_walk A w)%Z = 0%Z <->
+(finite_payoff_walk A w)%Z = 0%Z).
+{lia. } apply H0. apply initial_null. auto.
+Defined.
+
+Definition asynchronous_game_dual (G: AsynchronousGame) 
+: AsynchronousGame.
+  refine({| 
+            A := asynchronous_arena_dual (A G) ;
+            X := opposite_group (Y G);
+            Y := opposite_group (X G);
+            action g m h := action G h m g;
+         |}).
+Proof. 
+- simpl. apply action_id.
+- simpl. intros. apply action_compatible.
+- simpl. intros. apply coherence_1. auto.
+- simpl. intros. 
+assert (forall a b, negb a = negb b <-> a = b).
+{intros. destruct a; destruct b; intuition. }
+intros. apply H. apply coherence_2.
+- simpl. intros. rewrite negb_false_iff in H.
+apply coherence_4. auto.
+- simpl. intros. rewrite negb_true_iff in H.
+apply coherence_3. auto.
+- simpl. intros. apply action_preserves_initial.
+- simpl. intros. apply action_preserves_non_initial.
+Defined.
