Group.v
@@ -1,0 +1,115 @@
+Record Group := {
+      G : Type;
+      mult : G -> G -> G;
+      id : G;
+      inverse : G -> G;
+
+      associative : forall (x y z : G),
+      mult x (mult y z) = mult (mult x y) z;
+      id_exists : forall (x : G), 
+      mult id x = x /\ mult x id = x;
+      inverses_exist : forall (x : G),
+      mult x (inverse x) = id /\ mult (inverse x) x = id;
+}.
+
+Fact inverse_is_unique (G: Group) : forall x y z,
+mult G x y = id G /\ mult G x z = id G -> y = z.
+Proof. intros. destruct H. rewrite <- H in H0.
+assert (mult G (inverse G x) (mult G x z) = 
+mult G (inverse G x) (mult G x y) ).
+{  rewrite H0. reflexivity. }
+rewrite associative in H1. rewrite associative in H1.
+assert (mult G (inverse G x) x = id G).
+{ apply inverses_exist. }
+rewrite H2 in H1. 
+assert (mult G (id G) z = z /\ mult G (id G) y = y).
+{ split. 
++ apply id_exists.
++ apply id_exists. }
+destruct H3. rewrite H3 in H1. rewrite H4 in H1. auto.
+Qed.
+
+Fact mult_inverse (G: Group) : forall g g',
+mult G (inverse G g') (inverse G g) = inverse G (mult G g g').
+Proof. intros. 
+assert (mult G (mult G g g') (mult G (inverse G g') (inverse G g)) = id G /\
+mult G (mult G g g') (inverse G (mult G g g')) = id G).
+{ assert (mult G (mult G g g') (inverse G (mult G g g')) = id G).
+{ apply inverses_exist. }
+assert (mult G (mult G g g') (mult G (inverse G g') (inverse G g)) = id G).
+{ rewrite associative. 
+assert (mult G (mult G g g') (inverse G g') = g).
+{ rewrite <- associative.
+assert (mult G g' (inverse G g') = id G).
+{ apply inverses_exist. }
+rewrite H0. apply id_exists.
+  }
+rewrite H0. apply inverses_exist.
+ }
+rewrite H. rewrite H0. auto.
+} apply inverse_is_unique with (G0:=G) (x:=mult G g g')
+(y:=mult G (inverse G g') (inverse G g)) (z:=inverse G (mult G g g')).
+auto.
+Qed.
+
+Fact inverse_id_is_id (G: Group) : inverse G (id G) = id G.
+Proof. apply inverse_is_unique with (G0:=G) (x:=id G) 
+(y:= inverse G (id G)) (z:=id G). 
+split.
++ apply inverses_exist.
++ apply id_exists.
+Qed.
+
+Definition trivial_group : Group.
+refine({|
+          G := unit;
+          mult a b := tt;
+          id := tt
+      |}).
+Proof.
+- auto.
+- auto.
+- intros. destruct x. auto.
+- auto.
+Defined.
+
+Definition product_group (X Y : Group) : Group.
+refine ({|
+        G := (G X) * (G Y);
+        mult m n := (mult _ (fst m) (fst n), mult _ (snd m) (snd n));
+        id := (id _, id _);
+        inverse m := (inverse _ (fst m), inverse _ (snd m))
+       |}).
+Proof.
+- intros. destruct x. destruct y. destruct z. simpl.
+rewrite associative. rewrite associative. reflexivity.
+- intros. destruct x. simpl.
+assert (mult _ (id _) g = g /\ mult _ g (id _) = g).
+{ apply id_exists. }
+assert (mult _ (id _) g0 = g0 /\ mult _ g0 (id _) = g0).
+{ apply id_exists. }
+destruct H0. destruct H. rewrite H. rewrite H1. rewrite H0. rewrite H2. auto.
+- intros. destruct x. simpl. 
+assert (mult _ g (inverse _ g) = id _ /\ mult _ (inverse _ g) g = id _).
+{ apply inverses_exist. }
+assert (mult _ g0 (inverse _ g0) = id _ /\ mult _ (inverse _ g0) g0 = id _).
+{ apply inverses_exist. }
+destruct H. destruct H0. rewrite H. rewrite H1. rewrite H0. rewrite H2. auto.
+Defined.
+
+Definition opposite_group (X : Group) : Group.
+refine ({|
+        G := (G X) ;
+        mult m n := mult X n m;
+        id := id X;
+        inverse m := inverse X m
+       |}).
+Proof.
+- intros. rewrite associative. auto.
+- intros. split.
++ apply id_exists.
++ apply id_exists. 
+- intros. split.
++ apply inverses_exist.
++ apply inverses_exist.
+Defined.
