Lifting.v
@@ -1,0 +1,355 @@
+Require Import List.
+Require Import ZArith.
+Require Import Lia.
+Require Import Init.Nat.
+Require Import Logic.Eqdep.
+Require Import Logic.Eqdep_dec.
+Require Import Arith.PeanoNat.
+Require Import Bool.Bool.
+Require Import AsynchronousGames.
+
+Definition partial_order_lifting (P : PartialOrder) : PartialOrder.
+  refine({| 
+            I := unit;
+            N x := M P;
+            leq m n := match m,n with
+                       | existT _ tt (inl _), _ => True
+                       | existT _ tt (inr m), existT _ tt (inr n) => (leq P) m n
+                       | _, _ => False
+                       end;
+         |}).
+Proof. 
+- intros. destruct x. destruct x. destruct s.
+++ auto.
+++ apply reflexive.
+- intros. destruct x. destruct x. destruct H. destruct y. destruct x.
+destruct s.
++ destruct s0.
+++ destruct u. destruct u0. auto.
+++ contradiction H0.
++ destruct s0.
+++ contradiction H.
+++ assert (m = m0).
+{apply anti_symmetric. auto. } subst. auto.
+- intros. destruct x. destruct y. destruct z. destruct x. destruct x1.
+destruct x0. destruct H. destruct s.
++ destruct s0.
+++ auto.
+++ auto.
++ destruct s0.
+++ contradiction H.
+++ destruct s1.
++++ apply H0.
++++ apply transitive with (y:=m0). auto.
+- intros. destruct i. destruct i'. easy.
+- intros. destruct i. destruct i'. auto.
+Defined.
+
+Definition event_structure_lifting (E : EventStructure) : EventStructure.
+  refine({| 
+            P := partial_order_lifting (P E);
+            incompatible m n := match m,n with
+                                | existT _ tt (inr m), existT _ tt (inr n) => incompatible E m n
+                                | _, _ => False
+                                end;
+            ideal m := match m with
+                       | existT _ tt (inl tt) => (existT _ tt (inl tt)) :: nil
+                       | existT _ tt (inr m) =>
+                        (existT _ tt (inl tt)) :: (map (fun x => existT _ tt (inr x)) (ideal E m))
+                       end;
+         |}).
+Proof.
+- intros. destruct x. destruct y. destruct x. destruct x0. destruct s0.
++ destruct s;contradiction H.
++ destruct s.
+++ auto.
+++ apply symmetric. auto.
+- unfold not. intros. destruct x. destruct x. destruct s.
++ auto.
++ apply irreflexive in H. auto.
+- intros. destruct x. destruct y. destruct x. destruct x0. destruct s.
++ destruct s0.
+++ unfold iff. destruct u. destruct u0. split.
++++ intros. left. auto.
++++ intros. simpl. auto. 
+++ unfold iff. destruct u. split.
++++ intros. simpl in H. contradiction H.
++++ intros. destruct H; inversion H.
++ unfold iff. split.
+++ intros. destruct s0.
++++ left. destruct u. auto.
++++ right. simpl in H. apply ideal_finite in H.
+++++ apply in_map_iff. refine (ex_intro _ n0 _). auto.
+++ intros. destruct H.
++++ apply inj_pairT2 in H. subst. simpl. auto.
++++ apply in_map_iff in H. destruct H. destruct H.
+apply inj_pairT2 in H. subst. simpl. apply ideal_finite. auto.
+- intros. destruct x. destruct y. destruct z. destruct x.
+destruct x0. destruct x1. destruct s.
++ destruct H. contradiction H.
++ destruct s0.
+++ destruct H. contradiction H.
+++ destruct s1.
++++ simpl in H. destruct H. auto.
++++ simpl in H. apply incompatible_closed with (y:=n0). auto.
+Defined.
+
+Fixpoint cast_lifting E (l : Position (event_structure_lifting E))
+: Position E :=
+match l with
+| nil => nil
+| (existT _ tt (inl tt)) :: xs => cast_lifting E xs
+| (existT _ tt (inr m)) :: xs => m :: cast_lifting E xs
+end.
+
+Fixpoint cast_lifting_inf E (l : InfinitePosition (event_structure_lifting E))
+: InfinitePosition E :=
+match l with
+| stream _ (existT _ tt (inl tt)) f => cast_lifting_inf E (f tt)
+| stream _ (existT _ tt (inr m)) f =>
+stream _ m (fun _ => cast_lifting_inf E (f tt))
+end.
+
+Fact second_in_lifting_is_initial:
+forall E m, second_move (P (event_structure_lifting E)) m <->
+(exists i, m = existT _ tt (inr (existT _ i (inl tt)))).
+Proof. intros. unfold iff. split.
+- intros. unfold second_move in H. destruct m. destruct H.
+destruct s.
++ rewrite initial_is_unit in H. contradiction H. refine (ex_intro _ x _).
+destruct u. auto.
++ destruct x. destruct n.
+++ destruct s.
++++ destruct u. refine (ex_intro _ x _). auto.
++++ assert
+(initial_move (P (event_structure_lifting E)) 
+(existT
+          (fun i : I (P (event_structure_lifting E)) =>
+           (unit + N (P (event_structure_lifting E)) i)%type) tt
+          (inr (existT (fun i : I (P E) => (unit + N (P E) i)%type) x (inl tt))))).
+{apply H0. split.
++ simpl. apply unit_is_least. auto.
++ unfold not. intros. inversion H1. }
+rewrite initial_is_unit in H1. destruct H1. inversion H1.
+- intros. destruct H. subst. unfold second_move. split.
++ unfold not. intros. rewrite initial_is_unit in H. destruct H. inversion H.
++ intros. destruct H. destruct n.
+++ destruct x0. destruct s.
++++ simpl in H. rewrite initial_is_unit.
+refine (ex_intro _ tt _). destruct u. auto.
++++ simpl in H. destruct n.
+++++ assert (H1:=H). apply leq_same_component in H. subst.
+assert 
+((existT (fun i : I (P E) => (unit + N (P E) i)%type) x s) =
+       (existT (fun i : I (P E) => (unit + N (P E) i)%type) x (inl tt))).
+{apply anti_symmetric. split.
++ auto.
++ apply unit_is_least. auto. } apply inj_pairT2 in H. subst. contradiction H0.
+auto.
+Qed.
+
+Fixpoint contains_only_initial E (p : Position (event_structure_lifting E)) :=
+match p with
+| nil => false
+| existT _ tt (inl tt) :: nil => true
+| existT _ tt (inl tt) :: xs  => contains_only_initial E xs
+| _ => false
+end.
+
+Fixpoint cast_to_original E (p : Position (event_structure_lifting E)) :
+Position E :=
+match p with
+| nil => nil
+| existT _ tt (inl tt) :: xs => cast_to_original E xs
+| existT _ tt (inr m) :: xs => m :: (cast_to_original E xs)
+end.
+
+Fixpoint cast_inf_to_original E (p : InfinitePosition (event_structure_lifting E)) :
+InfinitePosition E :=
+match p with
+| stream _ (existT _ tt (inl tt)) f => cast_inf_to_original E (f tt)
+| stream _ (existT _ tt (inr m)) f =>
+stream _ m (fun _ => cast_inf_to_original E (f tt))
+end.
+
+Definition asynchronous_arena_lifting (A : AsynchronousArena) 
+(negative : (finite_payoff_position A) nil = (1)%Z)
+(p : Z)
+: AsynchronousArena.
+  refine({| 
+            E := event_structure_lifting (E A);
+            polarity m := match m with
+                          | existT _ tt (inl tt) => true
+                          | existT _ tt (inr m) => (polarity A) m
+                          end;
+            finite_payoff_position l :=
+              (match l with
+                | nil => (-1)%Z
+                | _ => if contains_only_initial _ l then p else
+                       finite_payoff_position A (cast_to_original _ l)
+              end);
+            finite_payoff_walk w :=
+              match w with
+                | ((_, nil), (_, nil)) => 0%Z
+                | ((_::_, _), (_::_, _)) =>
+                    let fp := cast_to_original _ (fst (fst w)) in
+                    let fm := cast_to_original _ (snd (fst w)) in
+                    let sp := cast_to_original _ (fst (snd w)) in
+                    let sm := cast_to_original _ (snd (snd w)) in
+                    finite_payoff_walk A ((fp, fm), (sp, sm)) 
+                | _ => finite_payoff_position A 
+                       (cast_to_original _ ((fst (snd w)) ++ (snd (snd w))))
+               end;
+            infinite_payoff l := infinite_payoff A (cast_inf_to_original _ l);
+         |}).
+Proof.
+- left. auto.
+- intros. destruct m. destruct x. destruct s.
++ destruct u. easy.
++ rewrite initial_is_unit in H. destruct H. inversion H.
+- intros. destruct m. destruct x. rewrite second_in_lifting_is_initial in H.
+destruct H. inversion H. subst. 
+assert (initial_move _ (existT (fun i : I (P (E A)) => (unit + N (P (E A)) i)%type) x
+      (inl tt)) ).
+{apply initial_is_unit. refine (ex_intro _ x _). auto. }
+apply polarity_first in H0. rewrite negative in H0. intuition.
+- intros. destruct w. destruct p0. destruct p1. simpl in *. destruct H. subst. simpl.
+destruct p0; destruct p1; auto.
+Defined.
+
+Definition asynchronous_game_lifting (G : AsynchronousGame) 
+(negative : (finite_payoff_position (A G)) nil = (1)%Z)
+(p : Z)
+: AsynchronousGame.
+  refine({| 
+             A := asynchronous_arena_lifting (A G) negative p;
+             X := X G;
+             Y := Y G;
+             action g m h := match m with
+                                | existT _ tt (inl tt) => m
+                                | existT _ tt (inr m) => 
+                                  existT _ tt (inr (action G g m h))
+                             end;
+        |}).
+Proof.
+- intros. destruct m. destruct x. destruct s.
++ destruct u. auto.
++ rewrite action_id. auto.
+- intros. destruct m. destruct x. destruct s.
++ destruct u. auto.
++ rewrite action_compatible. auto.
+- intros. destruct m. destruct x. destruct s.
++ destruct u. destruct n. simpl. auto.
++ simpl. simpl in H. destruct n. destruct x. destruct s.
+++ simpl. contradiction H.
+++ apply coherence_1. auto.
+- intros. destruct m. destruct x. destruct s.
++ destruct u. auto.
++ simpl. apply coherence_2.
+- intros. destruct m. destruct x. destruct s.
++ destruct u. auto.
++ simpl. simpl in H. destruct H. destruct n.
+++ 
+assert ((existT
+         (fun i : I (P (E (A G))) =>
+          (unit + N (P (E (A G))) i)%type) x s)
+ = (action G g
+        (existT
+           (fun i : I (P (E (A G))) =>
+            (unit + N (P (E (A G))) i)%type) x s) 
+        (id (Y G)))).
+{apply coherence_3. split.
++ auto.
++ intros. remember ((existT _ tt (inr n)) : 
+M (partial_order_lifting (P (E (A G))))) as n1.
+assert ((let (x0, s0) := n1 in
+      match x0 with
+      | tt =>
+          match s0 with
+          | inl _ => False
+          | inr n0 =>
+              leq (P (E (A G)))
+                (existT
+                   (fun i : I (P (E (A G))) =>
+                    (unit + N (P (E (A G))) i)%type) x s) n0
+          end
+      end) ->
+     n1 =
+     (let (x, s) := n1 in
+      match x with
+      | tt =>
+          fun s0 : unit + M (P (E (A G))) =>
+          match s0 with
+          | inl tt => n1
+          | inr m =>
+              existT
+                (fun _ : unit =>
+                 (unit + M (P (E (A G))))%type) tt
+                (inr (action G g m (id (Y G))))
+          end
+      end s)).
+{apply H0. } subst. simpl in *. apply H2 in H1.
+apply inj_pairT2 in H1. inversion H1. rewrite <- H4. auto.
+} rewrite <- H1. auto.
+- intros. destruct m. destruct x. destruct s.
++ destruct u. auto.
++ simpl in H. destruct n.
+++ simpl in H. destruct H. 
+assert (existT (fun i : I (P (E (A G))) => 
+(unit + N (P (E (A G))) i)%type) x s
+= action G (id (X G))
+        (existT (fun i : I (P (E (A G))) => 
+(unit + N (P (E (A G))) i)%type) x s) h).
+{apply coherence_4. split.
++ auto.
++ intros. remember ((existT _ tt (inr n)) : 
+M (partial_order_lifting (P (E (A G))))) as n1.
+assert ((let (x0, s0) := n1 in
+      match x0 with
+      | tt =>
+          match s0 with
+          | inl _ => False
+          | inr n0 =>
+              leq (P (E (A G)))
+                (existT
+                   (fun i : I (P (E (A G))) =>
+                    (unit + N (P (E (A G))) i)%type) x s) n0
+          end
+      end) ->
+     n1 =
+     (let (x, s) := n1 in
+      match x with
+      | tt =>
+          fun s0 : unit + M (P (E (A G))) =>
+          match s0 with
+          | inl tt => n1
+          | inr m =>
+              existT
+                (fun _ : unit => (unit + M (P (E (A G))))%type) tt
+                (inr (action G (id (X G)) m h))
+          end
+      end s)).
+{apply H0. } subst. simpl in H2. apply H2 in H1. 
+apply inj_pairT2 in H1. inversion H1. rewrite <- H4. auto. }
+rewrite <- H1. auto.
+- intros. destruct i. refine (ex_intro _ tt _). auto.
+- intros. destruct i. destruct m. destruct s.
++ destruct u. refine (ex_intro _ tt _).
+refine (ex_intro _
+((action G g
+          (existT (fun i : I (P (E (A G))) => (unit + N (P (E (A G))) i)%type) x (inl tt))
+          h)) _). auto.
++ refine (ex_intro _ tt _).
+refine (ex_intro _
+(action G g
+          (existT (fun i : I (P (E (A G))) => (unit + N (P (E (A G))) i)%type) x (inr n))
+          h) _). auto.
+Defined.
+
+Fact positive_lifting_is_positive :
+forall (G : AsynchronousGame) 
+(neg : (finite_payoff_position (A G)) nil = (1)%Z)
+(p : Z),
+finite_payoff_position 
+(A (asynchronous_game_lifting G neg p)) nil = (-1)%Z.
+Proof. intros. auto. Qed.
