Sum.v
@@ -1,0 +1,780 @@
+Require Import List.
+Require Import ZArith.
+Require Import Lia.
+Require Import Init.Nat.
+Require Import Logic.Eqdep.
+Require Import Logic.Eqdep_dec.
+Require Import Arith.PeanoNat.
+Require Import Bool.Bool.
+Require Import AsynchronousGames.
+Require Import Lifting.
+
+Inductive leq_sum (P Q : PartialOrder) :
+{i : I P + I Q & (sum unit (match i with
+                            | inl i => N P i
+                            | inr j => N Q j
+                            end))} ->
+{i : I P + I Q & (sum unit (match i with
+                            | inl i => N P i
+                            | inr j => N Q j
+                            end))} ->
+Prop :=
+| leq_sum_left : forall i m m' a b,
+leq P (existT _ i m) (existT _ i m') ->
+a = (existT _ (inl i) m) ->
+b = (existT _ (inl i) m') ->
+leq_sum P Q a b
+| leq_sum_right : forall i m m' a b,
+leq Q (existT _ i m) (existT _ i m') ->
+a = (existT _ (inr i) m) ->
+b = (existT _ (inr i) m') ->
+leq_sum P Q a b.
+
+Definition partial_order_sum (P Q : PartialOrder) : PartialOrder.
+  refine({| 
+            I := (I P) + (I Q);
+            N i := match i with
+                      | inl i => N P i
+                      | inr j => N Q j
+                   end;
+            leq := leq_sum P Q;
+         |}).
+Proof. 
+- intros. destruct x. destruct x. 
++ apply leq_sum_left with (i:=i) (m:=s) (m':=s).
+++ apply reflexive.
+++ auto.
+++ auto.
++ apply leq_sum_right with (i:=i) (m:=s) (m':=s).
+++ apply reflexive.
+++ auto.
+++ auto.
+- intros. destruct x. destruct y. destruct x.
++ destruct x0.
+++ destruct H. inversion H.
++++ subst. inversion H3. subst. apply inj_pairT2 in H3. subst.
+inversion H2. subst. apply inj_pairT2 in H2. subst. inversion H0.
+++++ subst. inversion H4. subst. apply inj_pairT2 in H4. subst.
+inversion H3. subst. apply inj_pairT2 in H3. subst.
+assert ((existT (fun i : I P => (unit + N P i)%type) i m'0)
+= (existT (fun i : I P => (unit + N P i)%type) i m0)).
+{apply anti_symmetric. auto. } apply inj_pairT2 in H3. subst. auto.
+++++ subst. inversion H4.
++++ subst. inversion H3.
+++ destruct H. inversion H.
++++ subst. inversion H3.
++++ subst. inversion H2.
++ destruct H. destruct x0.
+++ inversion H.
++++ subst. inversion H2.
++++ subst. inversion H3.
+++ inversion H.
++++ subst. inversion H3.
++++ subst. inversion H3. subst. apply inj_pairT2 in H3. subst.
+inversion H2. subst. apply inj_pairT2 in H2. subst. inversion H0.
+++++ subst. inversion H4.
+++++ subst. inversion H4. subst. apply inj_pairT2 in H4. subst.
+inversion H3. subst. apply inj_pairT2 in H3. subst.
+assert ((existT (fun i : I Q => (unit + N Q i)%type) i m0)
+        = (existT (fun i : I Q => (unit + N Q i)%type) i m'0)).
+{apply anti_symmetric. auto. }
+apply inj_pairT2 in H3. subst. auto.
+- intros. destruct x. destruct y. destruct z. destruct H. inversion H.
++ subst. inversion H3. subst. apply inj_pairT2 in H3. subst.
+inversion H2. subst. apply inj_pairT2 in H2. subst. inversion H0.
+++ subst. inversion H4. subst. apply inj_pairT2 in H4. subst. 
+inversion H3. subst. apply inj_pairT2 in H3. subst.
+assert (leq P (existT (fun i : I P => (unit + N P i)%type) i0 m)
+       (existT (fun i : I P => (unit + N P i)%type) i0 m'0)).
+{apply transitive with (y:=(existT (fun i : I P => (unit + N P i)%type) i0 m0)). auto. }
+apply leq_sum_left with (i:=i0) (m:=m) (m':=m'0). auto. auto. auto.
+++ subst. inversion H3. 
++ subst. inversion H3. subst. apply inj_pairT2 in H3. subst.
+inversion H2. subst. apply inj_pairT2 in H2. subst. inversion H0.
+++ subst. inversion H3.
+++ subst. inversion H3. subst. apply inj_pairT2 in H3. subst. inversion H4. subst.
+apply inj_pairT2 in H4. subst.
+assert ( leq Q (existT (fun i : I Q => (unit + N Q i)%type) i0 m)
+       (existT (fun i : I Q => (unit + N Q i)%type) i0 m'0)).
+{apply transitive with (y:=(existT (fun i : I Q => (unit + N Q i)%type) i0 m0)). auto. }
+apply leq_sum_right with (i:=i0) (m:=m) (m':=m'0). auto. auto. auto.
+- intros. unfold iff. split.
++ intros. inversion H. 
+++ subst. inversion H1. inversion H2. auto.
+++ subst. inversion H1. inversion H2. auto.
++ intros. subst. destruct i'.
+++ apply leq_sum_left with (i:=i) (m:=inl tt) (m':=m).
++++ apply unit_is_least. auto.
++++ auto.
++++ auto.
+++ apply leq_sum_right with (i:=i) (m:=inl tt) (m':=m).
++++ apply unit_is_least. auto.
++++ auto.
++++ auto.
+- intros. inversion H.
++ subst. inversion H1. inversion H2. subst. auto.
++ subst. inversion H1. inversion H2. subst. auto.
+Defined.
+
+Inductive incompatible_sum (E F : EventStructure) :
+(M (partial_order_sum (P E) (P F))) ->
+(M (partial_order_sum (P E) (P F))) ->
+Prop :=
+| incomp_sum_least : forall i i' m m',
+(i <> i') ->
+incompatible_sum E F (existT _ i m) (existT _ i' m')
+| incomp_sum_left : forall i m m' a b,
+incompatible E (existT _ i m) (existT _ i m') ->
+a = (existT _ (inl i) m) ->
+b = (existT _ (inl i) m') ->
+incompatible_sum E F a b
+| incomp_sum_right : forall i m m' a b,
+incompatible F (existT _ i m) (existT _ i m') ->
+a = (existT _ (inr i) m) ->
+b = (existT _ (inr i) m') ->
+incompatible_sum E F a b.
+
+Ltac flatten_all :=
+  repeat (let e := fresh "e" in
+      match goal with
+      | h: context[match ?x with | _ => _ end] |- _ => destruct x eqn:e
+      | |- context[match ?x with | _ => _ end] => destruct x eqn:e
+      end).
+
+Definition event_structure_sum (E F : EventStructure) : EventStructure.
+  refine({| 
+            P := partial_order_sum (P E) (P F);
+            incompatible := incompatible_sum E F;
+            ideal m := match m with
+                      | existT _ (inl i) m =>
+                      map (fun x => match x with
+                                    | existT _ i (inl tt) => existT _ (inl i) (inl tt)
+                                    | existT _ i (inr m) => existT _ (inl i) (inr m)
+                      end) (ideal E (existT _ i m))
+                      | existT _ (inr i) m =>
+                      map (fun x => match x with
+                                    | existT _ i (inl tt) => existT _ (inr i) (inl tt)
+                                    | existT _ i (inr m) => existT _ (inr i) (inr m)
+                      end) (ideal F (existT _ i m))
+                      end;
+         |}).
+Proof.
+- intros. inversion H.
++ subst. apply incomp_sum_least. auto.
++ subst. inversion H.
+++ subst. contradiction H2. auto.
+++ subst. inversion H2. subst. apply inj_pairT2 in H2. subst.
+apply inj_pairT2 in H3. subst. 
+apply incomp_sum_left with (m:=m'0) (m':=m0).
++++ apply symmetric. auto.
++++ auto.
++++ auto.
+++ subst. inversion H3.
++ subst. apply incomp_sum_right with (m:=m') (m':=m).
+++ apply symmetric. auto.
+++ auto.
+++ auto.
+- unfold not. intros. inversion H.
++ subst. contradiction H2. auto.
++ subst. apply inj_pairT2 in H2. subst.
+assert (~ incompatible E
+       (existT (fun i : I (P E) => (unit + N (P E) i)%type) i
+          m')
+       (existT (fun i : I (P E) => (unit + N (P E) i)%type) i
+          m')).
+{apply irreflexive. } contradiction H1.
++ subst. apply inj_pairT2 in H2. subst.
+assert (~ incompatible F
+       (existT (fun i : I (P F) => (unit + N (P F) i)%type) i
+          m')
+       (existT (fun i : I (P F) => (unit + N (P F) i)%type) i
+          m')).
+{apply irreflexive. } contradiction H1.
+- intros. simpl. flatten_all.
++ subst. unfold iff. split.
+++ intros. inversion H.
++++ subst. destruct m.
+++++ destruct m'.
++++++ apply in_map_iff.
+refine (ex_intro _ (existT _ i0 (inl tt)) _). split.
+++++++ destruct u. auto.
+++++++ inversion H2. subst. apply inj_pairT2 in H2. subst.
+apply ideal_finite. destruct u. destruct u0. auto.
++++++ inversion H2. subst. apply inj_pairT2 in H2. subst.
+apply in_map_iff.
+refine (ex_intro _ (existT _ i0 (inl tt)) _). split.
+++++++ destruct u. auto.
+++++++ apply ideal_finite. destruct u. auto.
+++++ inversion H2. subst. apply inj_pairT2 in H2. subst.
+apply in_map_iff.
+refine (ex_intro _ (existT _ i0 (inr n)) _). split.
++++++ auto.
++++++ apply ideal_finite. auto.
++++ subst. inversion H2.
+++ intros. apply in_map_iff in H. destruct H. destruct H.
+subst. destruct x. apply ideal_finite in H0.
+assert (H1 := H0). apply leq_same_component in H0. subst. destruct s0.
++++ destruct u. apply leq_sum_left with (i:=i) (m:=inl tt) (m':=s).
+++++ apply unit_is_least. auto.
+++++ auto.
+++++ auto.
++++ apply leq_sum_left with (i:=i) (m:=inr n) (m':=s).
+++++ auto.
+++++ auto.
+++++ auto.
++ subst. unfold iff. split.
+++ intros. inversion H.
++++ subst. inversion H2.
++++ subst. inversion H2. subst. apply inj_pairT2 in H2. subst.
+apply in_map_iff.
+refine (ex_intro _ (existT _ i0 m) _). split.
+++++ simpl. destruct m.
++++++ destruct u. auto.
++++++ auto.
+++++ apply ideal_finite. auto.
+++ intros. apply in_map_iff in H. destruct H. destruct H. subst.
+destruct x. apply ideal_finite in H0. assert (H1 := H0).
+apply leq_same_component in H0. subst. destruct s0.
++++ destruct u. apply leq_sum_right with (i:=i) (m:=inl tt) (m':=s); auto.
++++ apply leq_sum_right with (i:=i) (m:=inr n) (m':=s); auto.
+- intros. destruct H. inversion H.
++ subst. inversion H0; subst; inversion H3; subst; apply incomp_sum_least; auto.
++ subst. inversion H0.
+++ subst. inversion H3. subst. apply inj_pairT2 in H3. subst.
+apply incomp_sum_left with (i:=i0) (m:=m) (m':=m'0).
+apply incompatible_closed with (y:=existT (fun i : I (P E) => (unit + N (P E) i)%type) i0 m0).
+auto. auto. auto.
+++ subst. apply incomp_sum_least. easy.
++ subst. inversion H0.
+++ subst. apply incomp_sum_least. easy.
+++ subst. inversion H3. subst. apply inj_pairT2 in H3. subst.
+apply incomp_sum_right with (i:=i0) (m:=m) (m':=m'0).
+apply incompatible_closed with (existT (fun i : I (P F) => (unit + N (P F) i)%type) i0 m0).
+auto. auto. auto.
+Defined.
+
+Fixpoint cast_sum_to_left E F (l : Position (event_structure_sum E F))
+: Position E :=
+match l with
+| nil => nil
+| (existT _ (inl i) m) :: xs
+=> (existT _ i m) :: (cast_sum_to_left E F xs)
+| (existT _ (inr i) m) :: xs => cast_sum_to_left E F xs
+end.
+
+Fixpoint cast_sum_to_right E F (l : Position (event_structure_sum E F))
+: Position F :=
+match l with
+| nil => nil
+| (existT _ (inr i) m) :: xs
+=> (existT _ i m) :: (cast_sum_to_right E F xs)
+| (existT _ (inl i) m) :: xs => cast_sum_to_right E F xs
+end.
+
+Fixpoint cast_sum_inf_to_left E F (l : InfinitePosition (event_structure_sum E F))
+: InfinitePosition E :=
+match l with
+| stream _ (existT _ (inl i) m) f =>
+stream _ (existT _ i m) (fun _ => cast_sum_inf_to_left E F (f tt))
+| stream _ (existT _ _ _) f => cast_sum_inf_to_left E F (f tt)
+end.
+
+Fixpoint cast_sum_inf_to_right E F (l : InfinitePosition (event_structure_sum E F))
+: InfinitePosition F :=
+match l with
+| stream _ (existT _ (inr i) m) f =>
+stream _ (existT _ i m) (fun _ => cast_sum_inf_to_right E F (f tt))
+| stream _ (existT _ _ _) f => cast_sum_inf_to_right E F (f tt)
+end.
+
+Fact initial_in_sum_is_initial :
+forall E F m, initial_move (P (event_structure_sum E F)) m <->
+((exists i n, m = existT _ (inl i) n /\ initial_move (P E) (existT _ i n))
+\/
+(exists i n, m = existT _ (inr i) n /\ initial_move (P F) (existT _ i n))).
+Proof. unfold iff. split.
++ intros. rewrite initial_is_unit in H. destruct H. subst. destruct x.
+++ left. refine (ex_intro _ i _). refine (ex_intro _ (inl tt) _). split.
++++ auto.
++++ apply initial_is_unit. refine (ex_intro _ i _). auto.
+++ right. refine (ex_intro _ i _). refine (ex_intro _ (inl tt) _). split.
++++ auto.
++++ apply initial_is_unit. refine (ex_intro _ i _). auto.
++ intros. destruct H.
+++ destruct H. destruct H. destruct H. subst. rewrite initial_is_unit.
+rewrite initial_is_unit in H0. destruct H0. inversion H. subst. apply inj_pairT2 in H.
+subst. refine (ex_intro _ (inl x1) _). auto.
+++ destruct H. destruct H. destruct H. subst. rewrite initial_is_unit.
+rewrite initial_is_unit in H0. destruct H0. inversion H. subst. apply inj_pairT2 in H.
+subst. refine (ex_intro _ (inr x1) _). auto.
+Qed.
+
+Fact second_in_sum_is_second :
+forall E F m, second_move (P (event_structure_sum E F)) m <->
+((exists i n, m = existT _ (inl i) n /\ second_move (P E) (existT _ i n))
+\/
+(exists i n, m = existT _ (inr i) n /\ second_move (P F) (existT _ i n))).
+Proof. unfold iff. split.
++ intros. unfold second_move in H. destruct H. rewrite initial_is_unit in H.
+destruct m. destruct x.
+++ left. refine (ex_intro _ i _). refine (ex_intro _ s _). split.
++++ auto.
++++  unfold second_move. split.
+++++ rewrite initial_is_unit. unfold not. intros. destruct H1. inversion H1.
+subst. apply inj_pairT2 in H1. subst. contradiction H. refine (ex_intro _ (inl x) _).
+auto.
+++++ intros. destruct n. destruct H1. assert (H3 := H1). 
+apply leq_same_component in H1. subst.
+assert (initial_move (P (event_structure_sum E F)) 
+(existT _ (inl i) s0)).
+{apply H0. split.
++ simpl. apply leq_sum_left with (i:=i) (m:=s0) (m':=s). auto. auto. auto.
++ unfold not. intros. apply inj_pairT2 in H1. subst. contradiction H2. auto. }
+rewrite initial_is_unit. rewrite initial_is_unit in H1. destruct H1. inversion H1.
+subst. apply inj_pairT2 in H1. subst. refine (ex_intro _ i _). auto.
+++ right. refine (ex_intro _ i _). refine (ex_intro _ s _). split.
++++ auto.
++++  unfold second_move. split.
+++++ rewrite initial_is_unit. unfold not. intros. destruct H1. inversion H1.
+subst. apply inj_pairT2 in H1. subst. contradiction H. refine (ex_intro _ (inr x) _).
+auto.
+++++ intros. destruct n. destruct H1. assert (H3 := H1). 
+apply leq_same_component in H1. subst.
+assert (initial_move (P (event_structure_sum E F)) 
+(existT _ (inr i) s0)).
+{apply H0. split.
++ simpl. apply leq_sum_right with (i:=i) (m:=s0) (m':=s). auto. auto. auto.
++ unfold not. intros. apply inj_pairT2 in H1. subst. contradiction H2. auto. }
+rewrite initial_is_unit. rewrite initial_is_unit in H1. destruct H1. inversion H1.
+subst. apply inj_pairT2 in H1. subst. refine (ex_intro _ i _). auto.
++ intros. destruct H.
+++ destruct H. destruct H. destruct H. subst. unfold second_move in H0. unfold second_move.
+destruct H0. rewrite initial_is_unit in H. split.
++++ rewrite initial_is_unit. unfold not. intros. contradiction H. destruct H1.
+inversion H1. subst. apply inj_pairT2 in H1. subst. refine (ex_intro _ x _). auto.
++++ intros. destruct n. destruct H1. assert (H3 := H1).
+apply leq_same_component in H1. subst. inversion H3.
+++++ subst. inversion H5. subst. apply inj_pairT2 in H5. subst. apply inj_pairT2 in H4. subst.
+assert (initial_move (P E)
+(existT (fun i : I (P E) => (unit + N (P E) i)%type) i m)).
+{apply H0. split.
++ auto.
++ unfold not. intros. apply inj_pairT2 in H4. subst. contradiction H2. auto. }
+rewrite initial_is_unit in H4. rewrite initial_is_unit. destruct H4. inversion H4. subst.
+apply inj_pairT2 in H7. subst. refine (ex_intro _ (inl x) _). auto.
+++++ subst. inversion H5.
+++ destruct H. destruct H. destruct H. subst. unfold second_move in H0.
+destruct H0. unfold second_move. split.
++++ rewrite initial_is_unit in H. rewrite initial_is_unit. unfold not. intros.
+contradiction H. destruct H1. inversion H1. subst. apply inj_pairT2 in H1. subst.
+refine (ex_intro _ x _). auto.
++++ intros. destruct n. destruct H1. inversion H1.
+++++ subst. inversion H5.
+++++ subst. inversion H5. subst. apply inj_pairT2 in H5. subst. destruct x1.
++++++ inversion H4.
++++++
+assert (initial_move (P F)
+(existT (fun i : I (P F) => (unit + N (P F) i)%type) i0 s)).
+{apply H0. inversion H4. subst. apply inj_pairT2 in H4. subst. split.
++ auto.
++ unfold not. intros. apply inj_pairT2 in H4. subst. contradiction H2. auto. }
+rewrite initial_is_unit. rewrite initial_is_unit in H5. destruct H5.
+inversion H5. subst. apply inj_pairT2 in H5. subst. refine (ex_intro _ (inr x) _).
+auto.
+Defined.
+
+Definition inf_plus i j :=
+match i,j with
+| plus_infinity, plus_infinity => plus_infinity
+| _, _ => minus_infinity
+end.
+
+Definition asynchronous_arena_sum (A B : AsynchronousArena) 
+(positive1 : (finite_payoff_position A) nil = (-1)%Z)
+(positive2 : (finite_payoff_position B) nil = (-1)%Z)
+: AsynchronousArena.
+  refine({| 
+            E := event_structure_sum (E A) (E B);
+            polarity m := match m with
+                          | existT _ (inl i) m => (polarity A) (existT _ i m)
+                          | existT _ (inr i) m => (polarity B) (existT _ i m)
+                          end;
+            finite_payoff_position l := 
+                let left := (cast_sum_to_left (E A) (E B) l) in
+                if Nat.eqb (length l) (length left) then
+                finite_payoff_position A left else 
+                finite_payoff_position B (cast_sum_to_right (E A) (E B) l);
+            finite_payoff_walk w :=
+              let fp := cast_sum_to_left _ _ (fst (fst w)) in
+              let fm := cast_sum_to_left _ _ (snd (fst w)) in
+              let sp := cast_sum_to_left _ _ (fst (snd w)) in
+              let sm := cast_sum_to_left _ _ (snd (snd w)) in
+              if Nat.eqb (length fm) (length (snd (fst w))) &&
+                 Nat.eqb (length sm) (length (snd (snd w))) then
+              finite_payoff_walk A ((fp, fm), (sp, sm)) else
+              let fp := cast_sum_to_right _ _ (fst (fst w)) in
+              let fm := cast_sum_to_right _ _ (snd (fst w)) in
+              let sp := cast_sum_to_right _ _ (fst (snd w)) in
+              let sm := cast_sum_to_right _ _ (snd (snd w)) in
+              finite_payoff_walk B ((fp, fm), (sp, sm));
+             infinite_payoff l :=
+              let left := infinite_payoff A (cast_sum_inf_to_left _ _ l) in
+              let right := infinite_payoff B (cast_sum_inf_to_right _ _ l) in
+              inf_plus left right;
+         |}).
+Proof.
+- left. auto.
+- intros. flatten_all.
++ subst. split.
+++ intros. simpl. auto.
+++ intros. simpl. apply initial_in_sum_is_initial in H. destruct H.
++++ destruct H. destruct H. destruct H. inversion H. subst. apply inj_pairT2 in H.
+subst. apply polarity_first in H1. apply H1 in H0. auto.
++++ destruct H. destruct H. destruct H. inversion H.
++ subst. split.
+++ intros. subst. simpl. auto.
+++ intros. simpl. apply initial_in_sum_is_initial in H. destruct H.
++++ destruct H. destruct H. destruct H. inversion H.
++++ destruct H. destruct H. destruct H. inversion H. subst. apply inj_pairT2 in H.
+subst. apply polarity_first in H1. apply H1 in H0. lia.
+- intros. flatten_all.
++ subst. split.
+++ intros. simpl. apply second_in_sum_is_second in H. destruct H.
++++ destruct H. destruct H. destruct H. inversion H. subst. apply inj_pairT2 in H. subst.
+apply polarity_second in H1. apply H1 in H0. auto.
++++ destruct H. destruct H. destruct H. inversion H.
+++ intros. simpl. auto.
++ intros. simpl. split.
+++ intros. apply second_in_sum_is_second in H. destruct H.
++++ destruct H. destruct H. destruct H. inversion H.
++++ destruct H. destruct H. destruct H. inversion H. subst. apply inj_pairT2 in H. subst.
+apply polarity_second in H1. apply H1 in H0. auto. lia.
+++ intros. auto.
+- intros. destruct H. destruct w. destruct p. destruct p0. simpl in *. subst. simpl.
+apply initial_null. auto.
+Defined.
+
+Definition asynchronous_game_sum_positive (G H: AsynchronousGame) 
+(pos1 : (finite_payoff_position (A G)) nil = (-1)%Z)
+(pos2 : (finite_payoff_position (A H)) nil = (-1)%Z)
+: AsynchronousGame.
+  refine({| 
+             A := asynchronous_arena_sum (A G) (A H) pos1 pos2;
+             X := product_group (X G) (X H);
+             Y := product_group (Y G) (Y H);
+             action g m h := match m with
+                                | existT _ (inl i) m => 
+                                  (match action G (fst g) (existT _ i m) (fst h) with
+                                    | existT _ i m => existT _ (inl i) m
+                                  end)
+                                | existT _ (inr i) m => 
+                                  (match action H (snd g) (existT _ i m) (snd h) with
+                                    | existT _ i m => existT _ (inr i) m
+                                  end)
+                              end;
+        |}).
+Proof.
+- intros. flatten_all.
++ subst. simpl in e1. rewrite action_id in e1. inversion e1. subst. apply inj_pairT2 in e1.
+subst. auto.
++ subst. simpl in e1. rewrite action_id in e1. inversion e1. subst. apply inj_pairT2 in e1.
+subst. auto.
+- intros. destruct g. destruct h. destruct h'. destruct g'. 
+flatten_all; subst; simpl fst in *; simpl snd in *; inversion e2; subst;
+rewrite action_compatible in e1; apply inj_pairT2 in e2; subst; rewrite e3 in e1;
+rewrite e1 in e5; inversion e5; subst; apply inj_pairT2 in e5; subst; auto.
+- intros. destruct g. destruct h. simpl fst in *. flatten_all; simpl fst in *.
+simpl snd in *; subst; assert (H1:=H0); apply leq_same_component in H0; inversion H0; subst.
++ assert (leq _
+(action G g (existT (fun i : I (P (E (A G))) => (unit + N (P (E (A G))) i)%type) i0 s) g1)
+(action G g (existT (fun i : I (P (E (A G))) => (unit + N (P (E (A G))) i)%type) i0 s1) g1)).
+{apply coherence_1. inversion H1.
++ subst. inversion H4. subst. apply inj_pairT2 in H3. subst. apply inj_pairT2 in H4. subst. auto. 
++ subst. inversion H4. } rewrite e4 in H2. rewrite e1 in H2. simpl. assert (H3:=H2). 
+apply leq_same_component in H3. subst. apply leq_sum_left with (i:=x2) (m:=s0) (m':=s2). auto. auto. auto.
++ subst. inversion H0.
+++ subst. inversion H3.
+++ subst. inversion H2.
++ subst. inversion H0.
+++ subst. inversion H2.
+++ subst. inversion H3.
++ subst. simpl fst in *. simpl snd in *.
+assert (leq _
+(action H g0
+       (existT (fun i : I (P (E (A H))) => (unit + N (P (E (A H))) i)%type) i s)
+       g2)
+(action H g0
+       (existT (fun i : I (P (E (A H))) => (unit + N (P (E (A H))) i)%type) i0 s1)
+       g2)).
+{apply coherence_1. inversion H0.
++ subst. inversion H3.
++ subst. inversion H2. inversion H2. subst. apply inj_pairT2 in H2. subst. inversion H3. inversion H3.
+subst. apply inj_pairT2 in H3. subst. auto. }
+rewrite e4 in H1. rewrite e1 in H1. assert (H2:=H1). apply leq_same_component in H1. subst.
+simpl. apply leq_sum_right with (i:=x2) (m:=s0) (m':=s2). auto. auto. auto.
+- intros. destruct g. destruct h. flatten_all; simpl fst in *; simpl snd in *; subst.
++ simpl. rewrite <- e1. apply coherence_2.
++ simpl. rewrite <- e1. apply coherence_2.
+- intros. destruct g. flatten_all; simpl fst in *; simpl snd in *; subst; destruct H0.
++ remember ((existT
+          (fun i : I (P (E (asynchronous_arena_sum (A G) (A H) pos1 pos2))) =>
+           (unit + N (P (E (asynchronous_arena_sum (A G) (A H) pos1 pos2))) i)%type)
+          (inl i) s)).
+assert (s1 =
+     (let (x, m) := s1 in
+      match
+        x as x0
+        return
+          (unit + N (P (E (asynchronous_arena_sum (A G) (A H) pos1 pos2))) x0 ->
+           M (P (E (asynchronous_arena_sum (A G) (A H) pos1 pos2))))
+      with
+      | inl i =>
+          fun
+            m0 : unit +
+                 N (P (E (asynchronous_arena_sum (A G) (A H) pos1 pos2))) (inl i) =>
+          let (i0, m1) :=
+            action G (fst (g, g0))
+              (existT (fun i0 : I (P (E (A G))) => (unit + N (P (E (A G))) i0)%type)
+                 i m0) (fst (id (product_group (Y G) (Y H)))) in
+          existT
+            (fun i1 : I (P (E (asynchronous_arena_sum (A G) (A H) pos1 pos2))) =>
+             (unit + N (P (E (asynchronous_arena_sum (A G) (A H) pos1 pos2))) i1)%type)
+            (inl i0) m1
+      | inr i =>
+          fun
+            m0 : unit +
+                 N (P (E (asynchronous_arena_sum (A G) (A H) pos1 pos2))) (inr i) =>
+          let (i0, m1) :=
+            action H (snd (g, g0))
+              (existT (fun i0 : I (P (E (A H))) => (unit + N (P (E (A H))) i0)%type)
+                 i m0) (snd (id (product_group (Y G) (Y H)))) in
+          existT
+            (fun i1 : I (P (E (asynchronous_arena_sum (A G) (A H) pos1 pos2))) =>
+             (unit + N (P (E (asynchronous_arena_sum (A G) (A H) pos1 pos2))) i1)%type)
+            (inr i0) m1
+      end m)).
+{apply H1. apply reflexive. } subst. 
+destruct (action G (fst (g, g0))
+          (existT (fun i0 : I (P (E (A G))) => (unit + N (P (E (A G))) i0)%type) i s)
+          (fst (id (product_group (Y G) (Y H))))) eqn:eqn1. simpl fst in *. rewrite e1 in eqn1.
+inversion H2. inversion H2. subst. apply inj_pairT2 in H2. subst. inversion eqn1. subst.
+apply inj_pairT2 in eqn1. subst. auto.
++ remember ((existT
+          (fun i : I (P (E (asynchronous_arena_sum (A G) (A H) pos1 pos2))) =>
+           (unit + N (P (E (asynchronous_arena_sum (A G) (A H) pos1 pos2))) i)%type)
+          (inr i) s)).
+assert (s1 =
+     (let (x, m) := s1 in
+      match
+        x as x0
+        return
+          (unit + N (P (E (asynchronous_arena_sum (A G) (A H) pos1 pos2))) x0 ->
+           M (P (E (asynchronous_arena_sum (A G) (A H) pos1 pos2))))
+      with
+      | inl i =>
+          fun
+            m0 : unit +
+                 N (P (E (asynchronous_arena_sum (A G) (A H) pos1 pos2))) (inl i) =>
+          let (i0, m1) :=
+            action G (fst (g, g0))
+              (existT (fun i0 : I (P (E (A G))) => (unit + N (P (E (A G))) i0)%type) i
+                 m0) (fst (id (product_group (Y G) (Y H)))) in
+          existT
+            (fun i1 : I (P (E (asynchronous_arena_sum (A G) (A H) pos1 pos2))) =>
+             (unit + N (P (E (asynchronous_arena_sum (A G) (A H) pos1 pos2))) i1)%type)
+            (inl i0) m1
+      | inr i =>
+          fun
+            m0 : unit +
+                 N (P (E (asynchronous_arena_sum (A G) (A H) pos1 pos2))) (inr i) =>
+          let (i0, m1) :=
+            action H (snd (g, g0))
+              (existT (fun i0 : I (P (E (A H))) => (unit + N (P (E (A H))) i0)%type) i
+                 m0) (snd (id (product_group (Y G) (Y H)))) in
+          existT
+            (fun i1 : I (P (E (asynchronous_arena_sum (A G) (A H) pos1 pos2))) =>
+             (unit + N (P (E (asynchronous_arena_sum (A G) (A H) pos1 pos2))) i1)%type)
+            (inr i0) m1
+      end m)).
+{apply H1. apply reflexive. } subst.
+destruct (action H (snd (g, g0))
+          (existT (fun i0 : I (P (E (A H))) => (unit + N (P (E (A H))) i0)%type) i s)
+          (snd (id (product_group (Y G) (Y H))))) eqn:eqn1.
+simpl snd in *. rewrite e1 in eqn1. inversion eqn1. subst. apply inj_pairT2 in eqn1.
+subst. inversion H2. inversion H2. subst. apply inj_pairT2 in H2. auto.
+- intros. destruct h. flatten_all; simpl fst in *; subst; destruct H0.
++ remember ((existT
+          (fun i : I (P (E (asynchronous_arena_sum (A G) (A H) pos1 pos2))) =>
+           (unit + N (P (E (asynchronous_arena_sum (A G) (A H) pos1 pos2))) i)%type)
+          (inl i) s)).
+assert (s1 =
+     (let (x, m) := s1 in
+      match
+        x as x0
+        return
+          (unit + N (P (E (asynchronous_arena_sum (A G) (A H) pos1 pos2))) x0 ->
+           M (P (E (asynchronous_arena_sum (A G) (A H) pos1 pos2))))
+      with
+      | inl i =>
+          fun
+            m0 : unit +
+                 N (P (E (asynchronous_arena_sum (A G) (A H) pos1 pos2))) (inl i) =>
+          let (i0, m1) :=
+            action G (fst (id (product_group (X G) (X H))))
+              (existT (fun i0 : I (P (E (A G))) => (unit + N (P (E (A G))) i0)%type) i
+                 m0) (fst (g, g0)) in
+          existT
+            (fun i1 : I (P (E (asynchronous_arena_sum (A G) (A H) pos1 pos2))) =>
+             (unit + N (P (E (asynchronous_arena_sum (A G) (A H) pos1 pos2))) i1)%type)
+            (inl i0) m1
+      | inr i =>
+          fun
+            m0 : unit +
+                 N (P (E (asynchronous_arena_sum (A G) (A H) pos1 pos2))) (inr i) =>
+          let (i0, m1) :=
+            action H (snd (id (product_group (X G) (X H))))
+              (existT (fun i0 : I (P (E (A H))) => (unit + N (P (E (A H))) i0)%type) i
+                 m0) (snd (g, g0)) in
+          existT
+            (fun i1 : I (P (E (asynchronous_arena_sum (A G) (A H) pos1 pos2))) =>
+             (unit + N (P (E (asynchronous_arena_sum (A G) (A H) pos1 pos2))) i1)%type)
+            (inr i0) m1
+      end m)).
+{apply H1. apply reflexive. } subst. destruct
+(action G (fst (id (product_group (X G) (X H))))
+          (existT (fun i0 : I (P (E (A G))) => (unit + N (P (E (A G))) i0)%type) i s)
+          (fst (g, g0))) eqn:eqn1.
+simpl fst in *. rewrite e1 in eqn1. inversion eqn1. subst. apply inj_pairT2 in eqn1.
+apply inj_pairT2 in H5. subst. inversion H2. inversion H2. subst. apply inj_pairT2 in H2. auto.
++ simpl snd in *. remember
+((existT
+          (fun i : I (P (E (asynchronous_arena_sum (A G) (A H) pos1 pos2))) =>
+           (unit + N (P (E (asynchronous_arena_sum (A G) (A H) pos1 pos2))) i)%type)
+          (inr i) s)).
+assert (s1 =
+     (let (x, m) := s1 in
+      match
+        x as x0
+        return
+          (unit + N (P (E (asynchronous_arena_sum (A G) (A H) pos1 pos2))) x0 ->
+           M (P (E (asynchronous_arena_sum (A G) (A H) pos1 pos2))))
+      with
+      | inl i =>
+          fun
+            m0 : unit +
+                 N (P (E (asynchronous_arena_sum (A G) (A H) pos1 pos2))) (inl i) =>
+          let (i0, m1) :=
+            action G (fst (id (product_group (X G) (X H))))
+              (existT (fun i0 : I (P (E (A G))) => (unit + N (P (E (A G))) i0)%type) i
+                 m0) (fst (g, g0)) in
+          existT
+            (fun i1 : I (P (E (asynchronous_arena_sum (A G) (A H) pos1 pos2))) =>
+             (unit + N (P (E (asynchronous_arena_sum (A G) (A H) pos1 pos2))) i1)%type)
+            (inl i0) m1
+      | inr i =>
+          fun
+            m0 : unit +
+                 N (P (E (asynchronous_arena_sum (A G) (A H) pos1 pos2))) (inr i) =>
+          let (i0, m1) :=
+            action H (snd (id (product_group (X G) (X H))))
+              (existT (fun i0 : I (P (E (A H))) => (unit + N (P (E (A H))) i0)%type) i
+                 m0) (snd (g, g0)) in
+          existT
+            (fun i1 : I (P (E (asynchronous_arena_sum (A G) (A H) pos1 pos2))) =>
+             (unit + N (P (E (asynchronous_arena_sum (A G) (A H) pos1 pos2))) i1)%type)
+            (inr i0) m1
+      end m)).
+{apply H1. apply reflexive. } subst.
+destruct (action H (snd (id (product_group (X G) (X H))))
+          (existT (fun i0 : I (P (E (A H))) => (unit + N (P (E (A H))) i0)%type) i s)
+          (snd (g, g0))) eqn:eqn1. simpl snd in *. inversion H2. inversion H2. subst.
+apply inj_pairT2 in H2. subst. rewrite e1 in eqn1. inversion eqn1. subst. apply inj_pairT2 in eqn1.
+auto.
+- intros. destruct g. destruct h. destruct i; simpl fst; simpl snd.
++ destruct (action G g
+       (existT (fun i : I (P (E (A G))) => (unit + N (P (E (A G))) i)%type) i
+          (inl tt)) g1) eqn:eqn1. refine (ex_intro _ (inl x) _). flatten_all. 
+assert (existT
+         (fun i : I (P (E (A G))) =>
+          (unit + N (P (E (A G))) i)%type) x s = 
+existT
+      (fun i : I (P (E (A G))) =>
+       (unit + N (P (E (A G))) i)%type) x0 s0).
+{rewrite <- eqn1. rewrite <- e. auto. } inversion H0. subst. apply inj_pairT2 in H3. subst.
+assert (exists k,
+ action G g
+      (existT (fun i : I (P (E (A G))) => (unit + N (P (E (A G))) i)%type) i (inl tt)) g1 = 
+existT (fun i : I (P (E (A G))) => (unit + N (P (E (A G))) i)%type) k (inl tt)).
+{apply action_preserves_initial. }
+destruct H1. 
+assert (existT (fun i : I (P (E (A G))) => (unit + N (P (E (A G))) i)%type) x0 s0 = 
+existT (fun i : I (P (E (A G))) => (unit + N (P (E (A G))) i)%type) x (inl tt)).
+{rewrite <- e. rewrite <- H1. auto. } inversion H2. subst. apply inj_pairT2 in H2.
+subst. auto.
++ flatten_all.
+assert (exists k,
+action H g0
+      (existT (fun i : I (P (E (A H))) => (unit + N (P (E (A H))) i)%type) i (inl tt)) g2 = 
+existT (fun i : I (P (E (A H))) => (unit + N (P (E (A H))) i)%type) k (inl tt)).
+{apply action_preserves_initial. }
+destruct H0.
+assert (existT (fun i : I (P (E (A H))) => (unit + N (P (E (A H))) i)%type) x s = 
+     existT (fun i : I (P (E (A H))) => (unit + N (P (E (A H))) i)%type) x0 (inl tt)).
+{rewrite <- e. rewrite <- H0. auto. }
+inversion H1. subst. apply inj_pairT2 in H1. subst. refine (ex_intro _ (inr x0) _). auto.
+- intros. destruct i.
++ flatten_all. refine (ex_intro _ (inl x) _).
+assert (exists k k1,
+action G (fst g)
+      (existT (fun i : I (P (E (A G))) => (unit + N (P (E (A G))) i)%type) i (inr m))
+      (fst h) = 
+existT (fun i : I (P (E (A G))) => (unit + N (P (E (A G))) i)%type) k (inr k1)).
+{apply action_preserves_non_initial. }
+destruct H0. destruct H0. rewrite e in H0. inversion H0. subst. apply inj_pairT2 in H3. subst.
+refine (ex_intro _ x1 _). auto.
++ flatten_all. refine (ex_intro _ (inr x) _).
+assert (exists k k1,
+action H (snd g)
+      (existT (fun i : I (P (E (A H))) => (unit + N (P (E (A H))) i)%type) i (inr m))
+      (snd h) = 
+existT (fun i : I (P (E (A H))) => (unit + N (P (E (A H))) i)%type) k (inr k1)).
+{apply action_preserves_non_initial. }
+destruct H0. destruct H0. rewrite e in H0. inversion H0. subst. apply inj_pairT2 in H3. subst.
+refine (ex_intro _ x1 _). auto.
+Defined.
+
+Definition asynchronous_game_sum_left (G H: AsynchronousGame) 
+(neg : (finite_payoff_position (A G)) nil = (1)%Z)
+(pos : (finite_payoff_position (A H)) nil = (-1)%Z) : AsynchronousGame :=
+asynchronous_game_sum_positive
+(asynchronous_game_lifting G neg 0)
+H
+(positive_lifting_is_positive G neg 0)
+pos.
+
+Definition asynchronous_game_sum_right (G H: AsynchronousGame) 
+(pos : (finite_payoff_position (A G)) nil = (-1)%Z)
+(neg : (finite_payoff_position (A H)) nil = (1)%Z) : AsynchronousGame :=
+asynchronous_game_sum_positive
+G
+(asynchronous_game_lifting H neg 0)
+pos
+(positive_lifting_is_positive H neg 0).
+
+Definition asynchronous_game_sum_negative (G H: AsynchronousGame) 
+(neg1 : (finite_payoff_position (A G)) nil = (1)%Z)
+(neg2 : (finite_payoff_position (A H)) nil = (1)%Z) : AsynchronousGame :=
+asynchronous_game_sum_positive
+(asynchronous_game_lifting G neg1 0)
+(asynchronous_game_lifting H neg2 0)
+(positive_lifting_is_positive G neg1 0)
+(positive_lifting_is_positive H neg2 0).
+
+Definition asynchronous_game_sum (G H: AsynchronousGame) :
+AsynchronousGame :=
+match initial_payoff (A G), initial_payoff (A H) with
+| left p, left p' => asynchronous_game_sum_positive G H p p'
+| left p, right p' => asynchronous_game_sum_right G H p p'
+| right p, left p' => asynchronous_game_sum_left G H p p'
+| right p, right p' => asynchronous_game_sum_negative G H p p'
+end.
