Tensor.v
@@ -1,0 +1,1443 @@
+Require Import List.
+Require Import ZArith.
+Require Import Lia.
+Require Import Init.Nat.
+Require Import Logic.Eqdep.
+Require Import Logic.Eqdep_dec.
+Require Import Arith.PeanoNat.
+Require Import Bool.Bool.
+Require Import AsynchronousGames.
+Require Import Lifting.
+
+Inductive leq_tensor (P Q : PartialOrder) :
+{i : ((I P) * (I Q)) & (sum unit (sum (N P (fst i)) (N Q (snd i)))) } ->
+{i : ((I P) * (I Q)) & (sum unit (sum (N P (fst i)) (N Q (snd i)))) } ->
+Prop :=
+| leq_tensor_least : forall i j m, 
+leq_tensor P Q (existT _ (i, j) (inl tt)) (existT _ (i, j) m)
+| leq_tensor_left : forall i j m m' a b,
+leq P (existT _ i (inr m)) (existT _ i (inr m')) ->
+a = (existT _ (i, j) (inr (inl m))) ->
+b = (existT _ (i, j) (inr (inl m'))) ->
+leq_tensor P Q a b
+| leq_tensor_right : forall i j m m' a b, 
+leq Q (existT _ j (inr m)) (existT _ j (inr m')) -> 
+a = (existT _ (i, j) (inr (inr m))) ->
+b = (existT _ (i, j) (inr (inr m'))) ->
+leq_tensor P Q a b.
+
+Definition partial_order_tensor (P Q : PartialOrder) : PartialOrder.
+  refine({| 
+            I := (I P) * (I Q);
+            N x := sum (N P (fst x)) (N Q (snd x));
+            leq := leq_tensor P Q
+         |}).
+Proof. 
+- intros.
++ destruct x. destruct x. destruct s.
+++ destruct u. apply leq_tensor_least.
+++ destruct s.
++++ apply leq_tensor_left with (i:=i) (j:=i0) (m:=n) (m':=n).
+++++ apply reflexive.
+++++ auto.
+++++ auto.
++++ apply leq_tensor_right with (i:=i) (j:=i0) (m:=n) (m':=n).
+++++ apply reflexive.
+++++ auto.
+++++ auto.
+- intros. destruct x. destruct y. destruct H. inversion H.
++ subst. inversion H0.
+++ subst. apply inj_pairT2 in H3. subst. apply inj_pairT2 in H6.
+subst. apply inj_pairT2 in H5. subst. auto.
+++ subst. apply inj_pairT2 in H5. subst. inversion H2.
+subst. apply inj_pairT2 in H2. inversion H2. subst.
+apply inj_pairT2 in H3. subst. apply inj_pairT2 in H4. inversion H4.
+++ subst. apply inj_pairT2 in H5. subst. inversion H2. subst.
+apply inj_pairT2 in H2. subst. apply inj_pairT2 in H3. subst.
+apply inj_pairT2 in H4. inversion H4.
++ subst. inversion H3. subst. inversion H2. subst.
+apply inj_pairT2 in H2. subst. apply inj_pairT2 in H6. subst.
+auto. inversion H0.
+++ subst. inversion H5. subst. apply inj_pairT2 in H5.
+inversion H5. subst. apply inj_pairT2 in H4. inversion H4. subst.
+assert 
+((existT (fun i : I P => (unit + N P i)%type) i0 (inr m0)) =
+       (existT (fun i : I P => (unit + N P i)%type) i0 (inr m'0))).
+{apply anti_symmetric. auto. }
+apply inj_pairT2 in H6. inversion H6. auto.
+++ subst. inversion H5. 
++ subst. inversion H3. subst. inversion H2. subst.
+apply inj_pairT2 in H7. subst. apply inj_pairT2 in H3. subst.
+inversion H0.
+++ subst. inversion H5. 
+++ subst. inversion H5. subst. apply inj_pairT2 in H5. inversion H5.
+subst. apply inj_pairT2 in H4. inversion H4. subst.
+assert (
+(existT (fun i : I Q => (unit + N Q i)%type) j0 (inr m0)) = 
+(existT (fun i : I Q => (unit + N Q i)%type) j0 (inr m'0)) ).
+{ apply anti_symmetric. auto. }
+apply inj_pairT2 in H7. inversion H7. auto.
+- intros. destruct H. inversion H.
++ subst. inversion H0.
+++ subst. apply leq_tensor_least.
+++ subst. inversion H2. subst. apply leq_tensor_least.
+++ subst. inversion H2. subst. apply leq_tensor_least.
++ subst. inversion H0.
+++ subst. inversion H3. subst. apply inj_pairT2 in H3.
+inversion H3. subst.
+assert (leq P
+       (existT (fun i : I P => (unit + N P i)%type) i0 (inr m))
+       (existT (fun i : I P => (unit + N P i)%type) i0 (inr m'0))).
+{apply transitive with (y:=
+(existT (fun i : I P => (unit + N P i)%type) i0 (inr m0))). auto. }
+apply leq_tensor_left with (i:=i0) (j:=j0) (m:=m) (m':=m'0). auto.
+auto. auto.
+++ subst. inversion H3.
++ subst. inversion H0.
+++ subst. inversion H3.
+++ subst. inversion H3. subst. apply inj_pairT2 in H3. inversion H3.
+subst.
+assert (leq Q
+       (existT (fun i : I Q => (unit + N Q i)%type) j0 (inr m))
+       (existT (fun i : I Q => (unit + N Q i)%type) j0 (inr m'0))).
+{apply transitive with (y:=
+(existT (fun i : I Q => (unit + N Q i)%type) j0 (inr m0))). auto. }
+apply leq_tensor_right with (i:=i0) (j:=j0) (m:=m) (m':=m'0). auto.
+auto. auto.
+- intros. destruct i. unfold iff. split.
++ intros. inversion H.
+++ auto.
+++ subst. inversion H1.
+++ subst. inversion H1.
++ intros. subst. apply leq_tensor_least with (m:=m).
+- intros. inversion H.
++ auto.
++ subst. inversion H1. inversion H2. subst. auto.
++ subst. inversion H1. inversion H2. subst. auto.
+Defined.
+
+Inductive incompatible_tensor (E F : EventStructure) :
+(M (partial_order_tensor (P E) (P F))) ->
+(M (partial_order_tensor (P E) (P F))) ->
+Prop :=
+| incomp_tensor_least : forall i j i' j' m m',
+((i <> i') \/ (j <> j')) ->
+incompatible_tensor E F (existT _ (i, j) m) (existT _ (i', j') m')
+| incomp_tensor_left : forall index m m' a b,
+incompatible E (existT _ (fst index) (inr m)) 
+(existT _ (fst index) (inr m')) ->
+a = (existT _ index (inr (inl m))) ->
+b = (existT _ index (inr (inl m'))) ->
+incompatible_tensor E F a b
+| incomp_tensor_right : forall index m m' a b, 
+incompatible F (existT _ (snd index) (inr m)) 
+(existT _ (snd index) (inr m')) ->
+a = (existT _ index (inr (inr m))) ->
+b = (existT _ index (inr (inr m'))) ->
+incompatible_tensor E F a b.
+
+Definition event_structure_tensor (E F : EventStructure) : EventStructure.
+  refine({| 
+            P := partial_order_tensor (P E) (P F);
+            incompatible := incompatible_tensor E F;
+            ideal m := match m with
+                      | existT _ (i, j) (inl tt) => (existT _ (i, j) (inl tt)) :: nil
+                      | existT _ (i, j) (inr (inl m)) =>
+                      map (fun x => match x with
+                                    | existT _ i (inl tt) => existT _ (i, j) (inl tt)
+                                    | existT _ i (inr m) => existT _ (i, j) (inr (inl m))
+                      end) (ideal E (existT _ i (inr m)))
+                      | existT _ (i, j) (inr (inr m)) =>
+                      map (fun x => match x with
+                                    | existT _ j (inl tt) => existT _ (i, j) (inl tt)
+                                    | existT _ j (inr m) => existT _ (i, j) (inr (inr m))
+                                    end) (ideal F (existT _ j (inr m)))
+                      end;
+         |}).
+Proof.
+- intros. inversion H.
++ subst. apply incomp_tensor_least. intuition.
++ subst. inversion H.
+++ subst. inversion H4. subst. intuition.
+++ subst. inversion H3. subst. apply inj_pairT2 in H6. subst.
+apply inj_pairT2 in H2. inversion H2. subst.
+apply incomp_tensor_left with (m:=m'0) (m':=m0).
++++ apply symmetric. auto.
++++ auto.
++++ auto.
+++ subst. inversion H3.
++ subst. apply incomp_tensor_right with (m:=m') (m':=m).
+++ apply symmetric. auto.
+++ auto.
+++ auto.
+- unfold not. intros. inversion H.
++ subst. intuition.
++ subst. apply inj_pairT2 in H2. inversion H2. subst.
+assert (~ incompatible E
+       (existT (fun i : I (P E) => (unit + N (P E) i)%type)
+          (fst index) (inr m'))
+       (existT (fun i : I (P E) => (unit + N (P E) i)%type)
+          (fst index) (inr m'))).
+{apply irreflexive. } contradiction H1.
++ subst. apply inj_pairT2 in H2. inversion H2. subst.
+assert (~ incompatible F
+       (existT (fun i : I (P F) => (unit + N (P F) i)%type)
+          (snd index) (inr m'))
+       (existT (fun i : I (P F) => (unit + N (P F) i)%type)
+          (snd index) (inr m'))).
+{apply irreflexive. } contradiction H1.
+- intros. simpl. destruct x.
++ destruct x. destruct y.
+++ destruct x. destruct s.
++++ simpl. destruct u.
+++++ unfold iff. split.
++++++ intros. simpl. left. inversion H.
+++++++ subst. apply inj_pairT2 in H6. subst.
+apply inj_pairT2 in H3. subst. auto.
+++++++ subst. inversion H2.
+++++++ subst. inversion H2.
++++++ intros. destruct H.
+++++++ inversion H. subst. apply inj_pairT2 in H. subst.
+apply leq_tensor_least.
+++++++ contradiction H.
++++ destruct n.
+++++ simpl. unfold iff. split.
++++++ intros. apply in_map_iff. inversion H.
+++++++ subst. inversion H6. subst. 
+apply inj_pairT2 in H3. subst.
+refine (ex_intro _ (existT _ i (inl tt)) _). split.
++++++++ auto.
++++++++ apply ideal_finite. apply unit_is_least. auto.
+++++++ subst. inversion H2. subst. apply inj_pairT2 in H2.
+inversion H2. subst. inversion H1. subst. apply inj_pairT2 in H1.
+subst. refine (ex_intro _ (existT _ i3 (inr m)) _). split.
++++++++ auto.
++++++++ apply ideal_finite. auto.
+++++++ subst. inversion H2.
++++++ intros. apply in_map_iff in H. destruct H. destruct x. destruct s.
+++++++ destruct u. inversion H. subst. inversion H0. subst.
+apply inj_pairT2 in H0. subst. apply ideal_finite in H1. 
+apply unit_is_least in H1. subst. apply leq_tensor_least.
+++++++ destruct H. inversion H. subst. apply inj_pairT2 in H. subst.
+apply ideal_finite in H0. assert (H1 := H0).
+apply leq_same_component in H0. subst.
+apply leq_tensor_left with (i:=i) (j:=i2) (m:=n0) (m':=n). auto. auto.
+auto.
+++++ unfold iff. split.
++++++ intros. apply in_map_iff. inversion H.
+++++++ subst. apply inj_pairT2 in H3. subst.
+refine (ex_intro _ (existT _ i0 (inl tt)) _). split.
++++++++ auto.
++++++++ apply ideal_finite. apply unit_is_least. auto.
+++++++ subst. inversion H1. subst. apply inj_pairT2 in H1. subst.
+inversion H2.
+++++++ subst. inversion H2. subst. apply inj_pairT2 in H2. inversion H2.
+subst. inversion H1. subst. apply inj_pairT2 in H7. subst.
+refine (ex_intro _ (existT _ j (inr m)) _). split.
++++++++ auto.
++++++++ apply ideal_finite. auto.
++++++ intros.
+++++++ apply in_map_iff in H. destruct H. destruct x. destruct H. 
+apply ideal_finite in H0. assert (H1 := H0). apply leq_same_component in H0. subst.
+destruct s. 
++++++++ destruct u. inversion H. subst. apply inj_pairT2 in H. subst.
+apply leq_tensor_least.
++++++++ inversion H. subst. apply inj_pairT2 in H. subst.
+apply leq_tensor_right with (i:=i1) (j:=i2) (m:=n0) (m':=n). auto. auto. auto.
+- intros. destruct H. inversion H.
++ subst. inversion H0.
+++ apply incomp_tensor_least. auto.
+++ subst. inversion H3. subst. apply incomp_tensor_least. auto.
+++ subst. inversion H3. subst. apply incomp_tensor_least. auto.
++ subst. inversion H0.
+++ subst. inversion H3. subst. apply inj_pairT2 in H3. inversion H3.
+subst. apply incomp_tensor_left with (m:=m) (m':=m'0). apply incompatible_closed
+with (y:=(existT (fun i0 : I (P E) => (unit + N (P E) i0)%type)
+     (fst (i, j)) (inr m0))). auto. auto. auto.
+++ subst. inversion H3.
++ subst. inversion H0.
+++ subst. inversion H3.
+++ subst. inversion H3. subst. apply inj_pairT2 in H3. inversion H3.
+subst. apply incomp_tensor_right with (m:=m) (m':=m'0). apply incompatible_closed
+with (y:=(existT (fun i0 : I (P F) => (unit + N (P F) i0)%type)
+     (snd (i, j)) (inr m0))). auto. auto. auto.
+Defined.
+
+Fixpoint cast_tensor_to_left E F (l : Position (event_structure_tensor E F))
+: Position E :=
+match l with
+| nil => nil
+| (existT _ (i,j) (inl tt)) :: xs
+=> (existT _ i (inl tt)) :: (cast_tensor_to_left E F xs)
+| (existT _ (i,j) (inr (inl m))) :: xs
+=> (existT _ i (inr m)) :: (cast_tensor_to_left E F xs)
+| (existT _ i (inr (inr _))) :: xs
+=> cast_tensor_to_left E F xs
+end.
+
+Fixpoint cast_tensor_to_right E F (l : Position (event_structure_tensor E F))
+: Position F :=
+match l with
+| nil => nil
+| (existT _ (i,j) (inl tt)) :: xs
+=> (existT _ j (inl tt)) :: (cast_tensor_to_right E F xs)
+| (existT _ (i,j) (inr (inr m))) :: xs
+=> (existT _ j (inr m)) :: (cast_tensor_to_right E F xs)
+| (existT _ i (inr (inl _))) :: xs
+=> cast_tensor_to_right E F xs
+end.
+
+Fixpoint cast_tensor_inf_to_left E F (l : InfinitePosition (event_structure_tensor E F))
+: InfinitePosition E :=
+match l with
+| stream _ (existT _ (i, j) (inl tt)) f =>
+stream _ (existT _ i (inl tt)) (fun _ => cast_tensor_inf_to_left E F (f tt))
+| stream _ (existT _ (i, j) (inr (inl m))) f =>
+stream _ (existT _ i (inr m)) (fun _ => cast_tensor_inf_to_left E F (f tt))
+| stream _ (existT _ (i, j) (inr (inr _))) f =>
+cast_tensor_inf_to_left E F (f tt)
+end.
+
+Fixpoint cast_tensor_inf_to_right E F (l : InfinitePosition (event_structure_tensor E F))
+: InfinitePosition F :=
+match l with
+| stream _ (existT _ (i, j) (inl tt)) f =>
+stream _ (existT _ j (inl tt)) (fun _ => cast_tensor_inf_to_right E F (f tt))
+| stream _ (existT _ (i, j) (inr (inr m))) f =>
+stream _ (existT _ j (inr m)) (fun _ => cast_tensor_inf_to_right E F (f tt))
+| stream _ (existT _ (i, j) (inr (inl _))) f =>
+cast_tensor_inf_to_right E F (f tt)
+end.
+
+Definition tensor (p q : Z) :=
+if Z.ltb p 0 then 
+(if Z.ltb q 0 then Z.add p q else p)
+else
+(if Z.ltb q 0 then q else Z.add p q).
+
+Definition tensor_infinity (p q : Infinity) :=
+match p, q with
+| plus_infinity, plus_infinity => plus_infinity
+| _, _ => minus_infinity
+end.
+
+Fact initial_is_unit :
+forall E m, initial_move E m <->
+(exists i, m = existT _ i (inl tt)).
+Proof. unfold iff. split.
++ intros. unfold initial_move in H. destruct m. 
+refine (ex_intro _ x _). symmetry. apply H.
+apply unit_is_least. auto.
++ intros. unfold initial_move. intros. destruct H. subst.
+apply anti_symmetric. split.
+++ auto.
+++ destruct n. apply leq_same_component in H0. subst. 
+apply unit_is_least. auto.
+Qed.
+
+Fact second_in_tensor_is_second :
+forall E F m, second_move (P (event_structure_tensor E F)) m <->
+((exists i j k, m = existT _ (i,j) (inr (inl k)) /\ 
+second_move (P E) (existT _ i (inr k)))
+\/
+(exists i j k, m = existT _ (i,j) (inr (inr k)) /\ 
+second_move (P F) (existT _ j (inr k)))).
+Proof. unfold iff. split.
++ intros. unfold second_move in H. destruct H.
+rewrite initial_is_unit in H. destruct m. destruct s.
+++ contradiction H. refine (ex_intro _ x _). destruct u. auto.
+++ destruct x. destruct n.
++++ left. refine (ex_intro _ i _). refine (ex_intro _ i0 _).
+refine (ex_intro _ n _). split.
+++++ auto.
+++++ unfold second_move. unfold not. intros. split.
++++++ intros. rewrite initial_is_unit in H1. destruct H1.
+inversion H1.
++++++ intros. destruct n0.
+++++++ destruct s.
++++++++ destruct u. apply initial_is_unit.
+refine (ex_intro _ x _). auto.
++++++++ destruct H1. assert (H3 := H1).
+apply leq_same_component in H3. subst.
+assert (initial_move (P (event_structure_tensor E F))
+(existT
+          (fun i : I (P (event_structure_tensor E F)) =>
+           (unit + N (P (event_structure_tensor E F)) i)%type)
+          (i, i0) (inr (inl n0)))).
+{apply H0. split.
++ apply leq_tensor_left with (i:=i) (j:=i0) (m:=n0) (m':=n).
+++ auto.
+++ auto.
+++ auto.
++ unfold not. intros. apply inj_pairT2 in H3. inversion H3. subst.
+contradiction H2. auto. }
+apply initial_is_unit in H3. destruct H3. inversion H3.
++++ simpl. right. refine (ex_intro _ i _). refine (ex_intro _ i0 _).
+refine (ex_intro _ n _). split.
+++++ auto.
+++++ unfold second_move. split.
++++++ unfold not. intros. apply initial_is_unit in H1. destruct H1.
+inversion H1.
++++++ intros. destruct H1. assert (H3 := H1). destruct n0.
+++++++ apply leq_same_component in H3. subst. destruct s.
++++++++ apply initial_is_unit. destruct u. refine (ex_intro _ i0 _).
+auto.
++++++++
+assert (initial_move (P (event_structure_tensor E F))
+(existT
+          (fun i : I (P (event_structure_tensor E F)) =>
+           (unit + N (P (event_structure_tensor E F)) i)%type)
+          (i, i0) (inr (inr n0)))).
+{apply H0. split.
++ apply leq_tensor_right with (i:=i) (j:=i0) (m:=n0) (m':=n).
+++ auto.
+++ auto.
+++ auto.
++ unfold not. intros. apply inj_pairT2 in H3. inversion H3. subst.
+contradiction H2. auto.
+ } apply initial_is_unit in H3. destruct H3. inversion H3.
++ intros. destruct H. 
+++ destruct H. destruct H. destruct H. destruct H. subst. unfold second_move.
+split.
++++ unfold not. intros. apply initial_is_unit in H. destruct H. inversion H.
++++ intros. destruct H. unfold second_move in H0. destruct H0. destruct n.
+++++ destruct s.
++++++ apply initial_is_unit. destruct u. refine (ex_intro _ x2 _). auto.
++++++ inversion H.
+++++++ subst. inversion H5. subst. apply inj_pairT2 in H5. inversion H5.
+subst. inversion H4. subst. apply inj_pairT2 in H4. inversion H4. subst.
+assert (initial_move (P E) (existT (fun i : I (P E) => (unit + N (P E) i)%type) i
+          (inr m))).
+{apply H2. split.
++ auto.
++ unfold not. intros. apply inj_pairT2 in H6. inversion H6. subst. contradiction H1. auto.
+} apply initial_is_unit in H6. destruct H6. inversion H6.
+++++++ subst. inversion H5.
+++ destruct H. destruct H. destruct H. destruct H. subst. unfold second_move. split.
++++ unfold not. intros. apply initial_is_unit in H. destruct H. inversion H.
++++ intros. destruct H. unfold second_move in H0. destruct H0. destruct n.
+++++ destruct s.
++++++ apply initial_is_unit. destruct u. refine (ex_intro _ x2 _). auto.
++++++ inversion H.
+++++++ subst. inversion H5.
+++++++ subst. inversion H5. subst. apply inj_pairT2 in H5. inversion H5.
+subst. inversion H4. subst. apply inj_pairT2 in H4. inversion H4. subst.
+assert (initial_move (P F) (existT (fun i : I (P F) => (unit + N (P F) i)%type) j
+          (inr m))).
+{apply H2. split.
++ auto.
++ unfold not. intros. apply inj_pairT2 in H6. inversion H6. subst. contradiction H1. auto.
+} apply initial_is_unit in H6. destruct H6. inversion H6.
+Qed. 
+
+Definition asynchronous_arena_tensor (A B : AsynchronousArena) 
+(positive1 : (finite_payoff_position A) nil = (-1)%Z)
+(positive2 : (finite_payoff_position B) nil = (-1)%Z)
+: AsynchronousArena.
+  refine({| 
+            E := event_structure_tensor (E A) (E B);
+            polarity m := match m with
+                          | existT _ (i,j) (inl ll) => true
+                          | existT _ (i,j) (inr (inl m)) => (polarity A) (existT _ i (inr m))
+                          | existT _ (i,j) (inr (inr m)) => (polarity B) (existT _ j (inr m))
+                          end;
+            finite_payoff_position l :=
+              (match l with
+                | nil => (-1)%Z
+                | _ => let left := finite_payoff_position A (cast_tensor_to_left _ _ l) in
+                       let right := finite_payoff_position B (cast_tensor_to_right _ _ l) in
+                       tensor left right
+              end);
+            finite_payoff_walk w :=
+              let fp := cast_tensor_to_left _ _ (fst (fst w)) in
+              let fm := cast_tensor_to_left _ _ (snd (fst w)) in
+              let sp := cast_tensor_to_left _ _ (fst (snd w)) in
+              let sm := cast_tensor_to_left _ _ (snd (snd w)) in
+              let left := finite_payoff_walk A ((fp, fm), (sp, sm)) in
+              let fp := cast_tensor_to_right _ _ (fst (fst w)) in
+              let fm := cast_tensor_to_right _ _ (snd (fst w)) in
+              let sp := cast_tensor_to_right _ _ (fst (snd w)) in
+              let sm := cast_tensor_to_right _ _ (snd (snd w)) in
+              let right := finite_payoff_walk B ((fp, fm), (sp, sm)) in
+              tensor left right;
+            infinite_payoff l :=
+              let left := infinite_payoff A (cast_tensor_inf_to_left _ _ l) in
+              let right := infinite_payoff B (cast_tensor_inf_to_right _ _ l) in
+              tensor_infinity left right;
+         |}).
+Proof.
+- left. auto.
+- intros. apply initial_is_unit in H. destruct H. subst.
+destruct x. easy.
+- intros. apply second_in_tensor_is_second in H. destruct H.
++ destruct H. destruct H. destruct H. destruct H. subst. apply polarity_second in H0.
+rewrite positive1 in H0. auto.
++ destruct H. destruct H. destruct H. destruct H. subst. apply polarity_second in H0.
+rewrite positive2 in H0. auto.
+- intros. destruct H. destruct w. destruct p. destruct p0. simpl in *. subst. simpl.
+assert ((finite_payoff_walk A
+     (cast_tensor_to_left (E A) (E B) p, nil,
+     (cast_tensor_to_left (E A) (E B) p0, nil))) = 0%Z).
+{apply initial_null. auto. }
+assert ((finite_payoff_walk B
+     (cast_tensor_to_right (E A) (E B) p, nil,
+     (cast_tensor_to_right (E A) (E B) p0, nil))) = 0%Z).
+{apply initial_null. auto. }
+assert (forall a b f, a = 0%Z /\ b = 0%Z /\ f 0%Z 0%Z  = 0%Z
+-> f a b = 0%Z).
+{intros. destruct H1. destruct H2. subst. auto. }
+apply H1. auto.
+Defined.
+
+Definition asynchronous_game_tensor_positive (G H: AsynchronousGame) 
+(pos1 : (finite_payoff_position (A G)) nil = (-1)%Z)
+(pos2 : (finite_payoff_position (A H)) nil = (-1)%Z)
+: AsynchronousGame.
+  refine({| 
+             A := asynchronous_arena_tensor (A G) (A H) pos1 pos2;
+             X := product_group (X G) (X H);
+             Y := product_group (Y G) (Y H);
+             action g m h := match m with
+                                | existT _ (i,j) (inl tt) => 
+                                  (match action G (fst g) (existT _ i (inl tt)) (fst h),
+                                         action H (snd g) (existT _ j (inl tt)) (snd h) with
+                                    | existT _ i _, existT _ j _ => existT _ (i,j) (inl tt)
+                                  end)
+                                | existT _ (i,j) (inr (inl m)) => 
+                                  (match action G (fst g) (existT _ i (inr m)) (fst h),
+                                         action H (snd g) (existT _ j (inl tt)) (snd h) with
+                                    | existT _ i (inl tt), existT _ j _ => existT _ (i,j) (inl tt)
+                                    | existT _ i (inr m), existT _ j _ => existT _ (i,j) (inr (inl m))
+                                  end)
+                                | existT _ (i,j) (inr (inr m)) => 
+                                  (match action G (fst g) (existT _ i (inl tt)) (fst h),
+                                         action H (snd g) (existT _ j (inr m)) (snd h) with
+                                    | existT _ i _, existT _ j (inl tt) => existT _ (i,j) (inl tt)
+                                    | existT _ i _, existT _ j (inr m) => existT _ (i,j) (inr (inr m))
+                                  end)
+                             end;
+        |}).
+Proof.
+- intros. destruct m. destruct x. destruct s.
++ destruct u. rewrite action_id. rewrite action_id. simpl. auto.
++ destruct n.
+++ simpl in *. flatten_all.
++++ subst. rewrite action_id in e. inversion e.
++++ subst. rewrite action_id in e. inversion e. subst. rewrite action_id in e1.
+inversion e1. subst. auto.
+++ flatten_all.
++++ subst. simpl in e. rewrite action_id in e. inversion e. subst.
+rewrite action_id in e0. inversion e0.
++++ subst. simpl in e. rewrite action_id in e. inversion e. subst.
+rewrite action_id in e0. inversion e0. subst. apply inj_pairT2 in e0. inversion e0. subst.
+auto.
+- intros. destruct g. destruct g'. destruct h. destruct h'. flatten_all
++ subst. simpl in *. inversion e6. subst. inversion e5. subst. 
+apply inj_pairT2 in e5. subst.
+rewrite action_compatible in e3.
+rewrite action_compatible in e4. rewrite e6 in e3.
+assert (leq _
+(action G g (existT (fun i : I (P (E (A G))) => 
+(unit + N (P (E (A G))) i)%type) i1 (inl tt)) g5)
+(action G g (existT (fun i : I (P (E (A G))) => 
+(unit + N (P (E (A G))) i)%type) i1 s3) g5)).
+{apply coherence_1. apply unit_is_least. auto. } rewrite e3 in H0.
+rewrite e11 in H0. apply leq_same_component in H0. subst.
+rewrite e7 in e4.
+assert (leq _
+(action H g0 (existT (fun i : I (P (E (A H))) =>
+(unit + N (P (E (A H))) i)%type) i2 (inl tt)) g6)
+(action H g0 (existT (fun i : I (P (E (A H))) =>
+(unit + N (P (E (A H))) i)%type) i2 s4) g6)).
+{apply coherence_1. apply unit_is_least. auto. }
+rewrite e12 in H0. rewrite e4 in H0. apply leq_same_component in H0. subst. auto.
++ subst. simpl in *. inversion e5.
++ subst. simpl in *. inversion e5.
++ subst. simpl in *. inversion e5.
++ subst. simpl in *. inversion e5.
++ subst. simpl in *. inversion e6. subst.
+rewrite action_compatible in e3. rewrite action_compatible in H1. assert (exists k k1,
+action G g1 (existT (fun i : I (P (E (A G))) => (unit + N (P (E (A G))) i)%type) i (inr n0)) g3 =
+     existT (fun i : I (P (E (A G))) => (unit + N (P (E (A G))) i)%type) k (inr k1)).
+{apply action_preserves_non_initial. }
+destruct H0. destruct H0. rewrite e8 in H0. inversion H0.
++ subst. simpl in *. inversion e7. 
++ subst. simpl in *. inversion e7. 
++ subst. simpl in *. inversion e7.
++ subst. simpl in *. inversion e7.
++ subst. simpl in *. inversion e7. 
++ subst. simpl in *. inversion e6. subst. 
+assert (exists k k1,
+action G g
+        (existT (fun i : I (P (E (A G))) => (unit + N (P (E (A G))) i)%type) i1
+           (inr n3)) g5 =
+      existT (fun i : I (P (E (A G))) => (unit + N (P (E (A G))) i)%type) k
+        (inr k1)).
+{apply action_preserves_non_initial. }
+destruct H0. destruct H0. rewrite e14 in H0. inversion H0.
++ subst. simpl in *. inversion e6. subst. rewrite action_compatible in e3.
+assert (exists k k1,
+action G g1
+          (existT
+             (fun i : I (P (E (A G))) => (unit + N (P (E (A G))) i)%type) i
+             (inr n0)) g3 = 
+existT (fun i : I (P (E (A G))) => (unit + N (P (E (A G))) i)%type) k
+       (inr k1)
+).
+{apply action_preserves_non_initial. }
+destruct H0. destruct H0. rewrite H0 in e3.
+assert (exists k k1,
+action G g
+       (existT (fun i : I (P (E (A G))) => (unit + N (P (E (A G))) i)%type)
+          x (inr x2)) g5 = 
+existT (fun i : I (P (E (A G))) => (unit + N (P (E (A G))) i)%type) k
+       (inr k1)).
+{apply action_preserves_non_initial. }
+destruct H2. destruct H2. rewrite e3 in H2. inversion H2.
++ subst. simpl in *. inversion e7.
++ subst. simpl in *. inversion e7.
++ subst. simpl in *. inversion e6. subst. inversion e5. subst.
+rewrite action_compatible in e3.
+assert (exists k k1,
+action G g1
+       (existT (fun i : I (P (E (A G))) => (unit + N (P (E (A G))) i)%type)
+          i (inr n0)) g3 = 
+existT (fun i : I (P (E (A G))) => (unit + N (P (E (A G))) i)%type) k
+       (inr k1)).
+{apply action_preserves_non_initial. }
+destruct H0. destruct H0. rewrite e7 in H0. inversion H0.
++ subst. simpl in *. inversion e6.
++ subst. simpl in *. inversion e6.
++ subst. simpl in *. inversion e6.
++ subst. simpl in *. inversion e6.
++ subst. simpl in *. inversion e6.
++ subst. simpl in *. inversion e6. rewrite action_compatible in e3.
+assert (exists k k1,
+action G g
+        (existT
+           (fun i : I (P (E (A G))) => (unit + N (P (E (A G))) i)%type) i1
+           (inr n4)) g5 = 
+existT (fun i : I (P (E (A G))) => (unit + N (P (E (A G))) i)%type)
+        k (inr k1)
+).
+{apply action_preserves_non_initial. }
+destruct H0. destruct H0. rewrite e13 in H0. inversion H0.
++ subst. simpl in *. inversion e6. subst. apply inj_pairT2 in e6. inversion e6. subst. 
+rewrite action_compatible in e3. rewrite action_compatible in e5. rewrite e7 in e3.
+rewrite e13 in e3. inversion e3. subst. apply inj_pairT2 in e3. inversion e3. subst.
+rewrite e9 in e5. 
+assert (leq _
+(action H g0
+        (existT
+           (fun i : I (P (E (A H))) => (unit + N (P (E (A H))) i)%type)
+           i2 (inl tt)) g6)
+(action H g0
+       (existT
+          (fun i : I (P (E (A H))) => (unit + N (P (E (A H))) i)%type) i2
+          s4) g6)).
+{apply coherence_1. apply unit_is_least. auto. }
+rewrite e5 in H0. rewrite e15 in H0. apply leq_same_component in H0. subst. auto.
++ subst. simpl in *. inversion e6.
++ subst. simpl in *. inversion e6.
++ subst. simpl in *.
+assert (exists k k1,
+action H g2
+       (existT (fun i : I (P (E (A H))) => (unit + N (P (E (A H))) i)%type)
+          i0 (inr n0)) g4 = 
+existT (fun i : I (P (E (A H))) => (unit + N (P (E (A H))) i)%type) k
+       (inr k1)).
+{apply action_preserves_non_initial. }
+destruct H0. destruct H0. rewrite e9 in H0. inversion H0.
++ subst. simpl in *. inversion e7.
++ subst. simpl in *. inversion e7.
++ subst. simpl in *. inversion e7.
++ subst. simpl in *. inversion e7.
++ subst. simpl in *. inversion e7.
++ subst. simpl in *. inversion e7.
++ subst. simpl in *. inversion e7.
++ subst. simpl in *.
+assert (exists k k1,
+action H g0
+        (existT
+           (fun i : I (P (E (A H))) => (unit + N (P (E (A H))) i)%type) i2
+           (inr n3)) g6 =
+existT (fun i : I (P (E (A H))) => (unit + N (P (E (A H))) i)%type)
+        k (inr k1)).
+{apply action_preserves_non_initial. }
+destruct H0. destruct H0. rewrite e15 in H0. inversion H0.
++ subst. simpl in *. rewrite action_compatible in e4.
+assert (exists k k1,
+action H g2
+          (existT
+             (fun i : I (P (E (A H))) =>
+              (unit + N (P (E (A H))) i)%type) i0
+             (inr n0)) g4 =
+existT (fun i : I (P (E (A H))) => (unit + N (P (E (A H))) i)%type) k
+       (inr k1)).
+{apply action_preserves_non_initial. }
+destruct H0. destruct H0. rewrite H0 in e4. 
+assert (exists k k1,
+action H g0
+          (existT
+             (fun i : I (P (E (A H))) =>
+              (unit + N (P (E (A H))) i)%type) x
+             (inr x2)) g6 =
+existT (fun i : I (P (E (A H))) => (unit + N (P (E (A H))) i)%type) k
+       (inr k1)).
+{apply action_preserves_non_initial. }
+destruct H1. destruct H1. rewrite H1 in e4. inversion e4.
++ subst. simpl in *.
+assert (exists k k1,
+action H g2
+       (existT (fun i : I (P (E (A H))) => (unit + N (P (E (A H))) i)%type)
+          i0 (inr n0)) g4 = 
+existT (fun i : I (P (E (A H))) => (unit + N (P (E (A H))) i)%type) k
+       (inr k1)).
+{apply action_preserves_non_initial. }
+destruct H0. destruct H0. rewrite e8 in H0. inversion H0.
++ subst. simpl in *. inversion e6.
++ subst. simpl in *. inversion e6.
++ subst. simpl in *. inversion e6.
++ subst. simpl in *. inversion e6.
++ subst. simpl in *. inversion e6.
++ subst. simpl in *. inversion e6.
++ subst. simpl in *. inversion e6.
++ subst. simpl in *. 
+assert (exists k k1,
+action H g0
+        (existT
+           (fun i : I (P (E (A H))) => (unit + N (P (E (A H))) i)%type) i2
+           (inr n4)) g6 =
+existT (fun i : I (P (E (A H))) => (unit + N (P (E (A H))) i)%type)
+        k (inr k1)).
+{apply action_preserves_non_initial. }
+destruct H0. destruct H0. rewrite e14 in H0. inversion H0.
++ subst. simpl in *. rewrite action_compatible in e3. inversion e6. subst.
+apply inj_pairT2 in e6. inversion e6. subst. rewrite action_compatible in e4.
+rewrite e8 in e4. rewrite e7 in e3. rewrite e4 in e14. inversion e14. subst.
+apply inj_pairT2 in e14. inversion e14. subst.
+assert (leq _
+(action G g
+        (existT
+           (fun i : I (P (E (A G))) =>
+            (unit + N (P (E (A G))) i)%type) i1
+           (inl tt)) g5)
+(action G g
+       (existT
+          (fun i : I (P (E (A G))) =>
+           (unit + N (P (E (A G))) i)%type) i1 s3) g5)).
+{apply coherence_1. apply unit_is_least. auto. }
+rewrite e13 in H0. rewrite e3 in H0. apply leq_same_component in H0. subst. auto.
+- intros. destruct g. destruct h. flatten_all; subst; simpl in *; try (
+inversion H0; subst; inversion H2; try (subst; inversion H3 )).
++ inversion H0.
+++ subst. apply inj_pairT2 in H6. subst. rewrite e3 in e9. inversion e9. subst.
+apply inj_pairT2 in e9. subst. rewrite e4 in e10. inversion e10. subst. apply inj_pairT2 in e10.
+subst. auto. apply leq_tensor_least.
+++ subst. inversion H2.
+++ subst. inversion H2.
++ assert (exists k k1, action G g
+       (existT (fun i : I (P (E (A G))) => (unit + N (P (E (A G))) i)%type)
+          i1 (inr n1)) g1 = 
+existT (fun i : I (P (E (A G))) => (unit + N (P (E (A G))) i)%type) k
+       (inr k1)).
+{apply action_preserves_non_initial. }
+destruct H1. destruct H1. rewrite e9 in H1. inversion H1.
++ inversion H0.
+++ subst.
+assert (leq _ (action G g
+       (existT
+          (fun i : I (P (E (A G))) => (unit + N (P (E (A G))) i)%type) i1
+          (inl tt)) g1) (action G g
+       (existT
+          (fun i : I (P (E (A G))) => (unit + N (P (E (A G))) i)%type) i1
+          (inr n1)) g1 )).
+{apply coherence_1. apply unit_is_least. auto. }
+rewrite e9 in H1. rewrite e3 in H1. assert (H2 := H1).
+apply leq_same_component in H1. subst. rewrite e4 in e11. inversion e11. subst.
+apply leq_tensor_least.
+++ subst. inversion H2.
+++ subst. inversion H2.
++ inversion H0.
+++ subst. rewrite e3 in e9. inversion e9. subst.
+assert (leq _ (action H g0
+       (existT (fun i : I (P (E (A H))) => (unit + N (P (E (A H))) i)%type) i2
+          (inl tt)) g2) (action H g0
+        (existT (fun i : I (P (E (A H))) => (unit + N (P (E (A H))) i)%type) i2
+           (inr n1)) g2)).
+{apply coherence_1. apply unit_is_least. auto. }
+rewrite e10 in H1. rewrite e4 in H1. apply leq_same_component in H1. subst. 
+apply leq_tensor_least.
+++ subst. inversion H3.
+++ subst. inversion H2. 
++ inversion H0.
+++ subst. rewrite e3 in e9. inversion e9. subst.
+assert (leq _ (action H g0
+       (existT (fun i : I (P (E (A H))) => (unit + N (P (E (A H))) i)%type) i2
+          (inl tt)) g2) (action H g0
+        (existT (fun i : I (P (E (A H))) => (unit + N (P (E (A H))) i)%type) i2
+           (inr n1)) g2)).
+{apply coherence_1. apply unit_is_least. auto. }
+rewrite e10 in H1. rewrite e4 in H1. apply leq_same_component in H1. subst. 
+apply leq_tensor_least.
+++ subst. inversion H3.
+++ subst. inversion H2.
++ inversion H0.
+++ subst. inversion H3.
+assert (exists k k1,
+action G g
+        (existT (fun i : I (P (E (A G))) => (unit + N (P (E (A G))) i)%type) i3
+           (inr n3)) g1
+= existT (fun i : I (P (E (A G))) => (unit + N (P (E (A G))) i)%type) k
+        (inr k1)).
+{apply action_preserves_non_initial. }
+destruct H6. destruct H6. rewrite e11 in H6. inversion H6.
+++ subst. inversion H2.
+assert (exists k k1,
+action G g
+        (existT (fun i : I (P (E (A G))) => (unit + N (P (E (A G))) i)%type) i3
+           (inr n3)) g1
+= existT (fun i : I (P (E (A G))) => (unit + N (P (E (A G))) i)%type) k
+        (inr k1)).
+{apply action_preserves_non_initial. }
+destruct H6. destruct H6. rewrite e11 in H6. inversion H6.
++ inversion H0.
+++ subst. inversion H2. subst. inversion H3. subst.
+assert (exists k k1,
+action G g
+        (existT (fun i : I (P (E (A G))) => (unit + N (P (E (A G))) i)%type) i3
+           (inr n1)) g1
+= existT (fun i : I (P (E (A G))) => (unit + N (P (E (A G))) i)%type) k
+        (inr k1)).
+{apply action_preserves_non_initial. }
+destruct H9. destruct H9. rewrite e3 in H9. inversion H9.
+++ subst. inversion H2.
+assert (exists k k1,
+action G g
+        (existT (fun i : I (P (E (A G))) => (unit + N (P (E (A G))) i)%type) i3
+           (inr n1)) g1
+= existT (fun i : I (P (E (A G))) => (unit + N (P (E (A G))) i)%type) k
+        (inr k1)).
+{apply action_preserves_non_initial. }
+destruct H6. destruct H6. rewrite e3 in H6. inversion H6.
+
++ inversion H0.
+++ subst. inversion H2. subst. inversion H3.
+assert (exists k k1,
+ action G g
+        (existT (fun i : I (P (E (A G))) => (unit + N (P (E (A G))) i)%type)
+           i3 (inr n4)) g1 = 
+existT (fun i : I (P (E (A G))) => (unit + N (P (E (A G))) i)%type) k
+        (inr k1)).
+{apply action_preserves_non_initial. }
+destruct H9. destruct H9. rewrite e10 in H9. inversion H9.
+++ assert (exists k k1,
+action G g
+        (existT (fun i : I (P (E (A G))) => (unit + N (P (E (A G))) i)%type)
+           i1 (inr n4)) g1 = 
+existT (fun i : I (P (E (A G))) => (unit + N (P (E (A G))) i)%type) k
+        (inr k1)).
+{apply action_preserves_non_initial. }
+destruct H11. destruct H11. rewrite e10 in H11. inversion H11.
++ inversion H0.
+++ subst. inversion H2. subst. inversion H5. apply inj_pairT2 in H5. inversion H5. subst.
+inversion H6. subst. apply inj_pairT2 in H6. inversion H6. subst. auto.
+inversion H8. subst. apply inj_pairT2 in H8. inversion H8. subst. apply inj_pairT2 in H7.
+inversion H7. subst. apply inj_pairT2 in H3. inversion H3. subst.
+assert (leq _
+(action G g (existT (fun i : I (P (E (A G))) => (unit + N (P (E (A G))) i)%type) i (inr m0)) g1)
+(action G g
+        (existT
+           (fun i : I (P (E (A G))) =>
+            (unit + N (P (E (A G))) i)%type) i 
+           (inr m')) g1)).
+{apply coherence_1. auto. }
+rewrite e10 in H9. rewrite e3 in H9. assert (H10 := H9). apply leq_same_component in H10. subst.
+rewrite e5 in e12. inversion e12. subst.
+apply leq_tensor_left with (i:=x3) (j:=x4) (m:=n2) (m':=n5). auto. auto. auto.
+++ subst. inversion H2. inversion H7.
++ inversion H0.
+++ subst. inversion H2. subst. inversion H3. inversion H8.
+++ subst. inversion H2.
+assert (exists k k1,
+action H g0
+       (existT (fun i : I (P (E (A H))) => (unit + N (P (E (A H))) i)%type) j (inr n1)) g2 = 
+existT (fun i : I (P (E (A H))) => (unit + N (P (E (A H))) i)%type) k (inr k1)).
+{apply action_preserves_non_initial. }
+destruct H6. destruct H6. rewrite e4 in H6. inversion H6.
++ inversion H0.
+++ subst. inversion H2. subst. inversion H3. subst. inversion H7.
+++ subst.
+assert (exists k k1,
+action H g0
+       (existT (fun i : I (P (E (A H))) => (unit + N (P (E (A H))) i)%type) j
+          (inr n1)) g2 = 
+existT (fun i : I (P (E (A H))) => (unit + N (P (E (A H))) i)%type) k
+       (inr k1)).
+{apply action_preserves_non_initial. }
+destruct H5. destruct H5. rewrite e4 in H5. inversion H5.
++ inversion H0.
+++ subst. inversion H2. subst. inversion H3. subst. inversion H7.
+++ subst.
+assert (exists k k1,
+action H g0
+       (existT (fun i : I (P (E (A H))) => (unit + N (P (E (A H))) i)%type) j
+          (inr n4)) g2 = 
+existT (fun i : I (P (E (A H))) => (unit + N (P (E (A H))) i)%type) k
+       (inr k1)).
+{apply action_preserves_non_initial. }
+destruct H5. destruct H5. rewrite e11 in H5. inversion H5.
++ inversion H0.
+++ subst. inversion H2. subst. inversion H3. subst. inversion H7.
+++ subst. inversion H8. subst. apply inj_pairT2 in H8. inversion H8. subst.
+apply inj_pairT2 in H7. inversion H7. subst. apply inj_pairT2 in H3. inversion H3. subst. rewrite e3 in e10.
+inversion e10. subst.
+assert (leq _
+(action H g0
+       (existT (fun i : I (P (E (A H))) => (unit + N (P (E (A H))) i)%type) j0
+          (inr m0)) g2)
+(action H g0
+        (existT (fun i : I (P (E (A H))) => (unit + N (P (E (A H))) i)%type) j0
+           (inr m')) g2)).
+{apply coherence_1. auto. }
+rewrite e11 in H5. rewrite e4 in H5. assert (H6 := H5). apply leq_same_component in H6. subst.
+apply leq_tensor_right with (i:=x3) (j:=x4) (m:=n2) (m':=n5). auto. auto. auto.
+- intros. destruct g. destruct h. flatten_all; subst; simpl in *.
++ auto.
++ assert (exists k k1,
+action G g
+       (existT (fun i : I (P (E (A G))) => (unit + N (P (E (A G))) i)%type) i
+          (inr n0)) g1 = 
+existT (fun i : I (P (E (A G))) => (unit + N (P (E (A G))) i)%type) k
+       (inr k1)).
+{apply action_preserves_non_initial. }
+destruct H0. destruct H0. rewrite e3 in H0. inversion H0.
++ rewrite <- e3. apply coherence_2.
++ assert (exists k k1,
+action H g0
+       (existT (fun i : I (P (E (A H))) => (unit + N (P (E (A H))) i)%type) i0
+          (inr n0)) g2 = 
+existT (fun i : I (P (E (A H))) => (unit + N (P (E (A H))) i)%type) k
+       (inr k1)).
+{apply action_preserves_non_initial. }
+destruct H0. destruct H0. rewrite e4 in H0. inversion H0.
++ rewrite <- e4. apply coherence_2.
+- intros. destruct g. flatten_all; subst; simpl in *; destruct H0.
++ inversion H0.
++ assert (exists k k1,
+action G g
+       (existT (fun i : I (P (E (A G))) => (unit + N (P (E (A G))) i)%type) i
+          (inr n0)) (id (Y G)) = 
+existT (fun i : I (P (E (A G))) => (unit + N (P (E (A G))) i)%type) k
+       (inr k1)).
+{apply action_preserves_non_initial. }
+destruct H2. destruct H2. rewrite e3 in H2. inversion H2.
++ remember (existT
+          (fun i : I (P (E (A G))) * I (P (E (A H))) =>
+           (unit +
+            (N (P (E (A G))) (fst i) +
+             N (P (E (A H))) (snd i)))%type) 
+          (i, i0) (inr (inl n0))).
+ assert ( s =
+     (let (x, s) := s in
+      (let
+         (i, j) as x0
+          return
+            (unit + (N (P (E (A G))) (fst x0) + N (P (E (A H))) (snd x0)) ->
+             M (partial_order_tensor (P (E (A G))) (P (E (A H))))) := x in
+       fun s0 : unit + (N (P (E (A G))) i + N (P (E (A H))) j) =>
+       match s0 with
+       | inl tt =>
+           let (i0, _) :=
+             action G g
+               (existT (fun i0 : I (P (E (A G))) => (unit + N (P (E (A G))) i0)%type) i (inl tt))
+               (id (Y G)) in
+           let (j0, _) :=
+             action H g0
+               (existT (fun i1 : I (P (E (A H))) => (unit + N (P (E (A H))) i1)%type) j (inl tt))
+               (id (Y H)) in
+           existT
+             (fun i1 : I (P (E (A G))) * I (P (E (A H))) =>
+              (unit + (N (P (E (A G))) (fst i1) + N (P (E (A H))) (snd i1)))%type) 
+             (i0, j0) (inl tt)
+       | inr (inl m) =>
+           let (i0, s1) :=
+             action G g
+               (existT (fun i0 : I (P (E (A G))) => (unit + N (P (E (A G))) i0)%type) i (inr m))
+               (id (Y G)) in
+           match s1 with
+           | inl tt =>
+               let (j0, _) :=
+                 action H g0
+                   (existT (fun i1 : I (P (E (A H))) => (unit + N (P (E (A H))) i1)%type) j
+                      (inl tt)) (id (Y H)) in
+               existT
+                 (fun i1 : I (P (E (A G))) * I (P (E (A H))) =>
+                  (unit + (N (P (E (A G))) (fst i1) + N (P (E (A H))) (snd i1)))%type) 
+                 (i0, j0) (inl tt)
+           | inr m0 =>
+               let (j0, _) :=
+                 action H g0
+                   (existT (fun i1 : I (P (E (A H))) => (unit + N (P (E (A H))) i1)%type) j
+                      (inl tt)) (id (Y H)) in
+               existT
+                 (fun i1 : I (P (E (A G))) * I (P (E (A H))) =>
+                  (unit + (N (P (E (A G))) (fst i1) + N (P (E (A H))) (snd i1)))%type) 
+                 (i0, j0) (inr (inl m0))
+           end
+       | inr (inr m) =>
+           let (i0, _) :=
+             action G g
+               (existT (fun i0 : I (P (E (A G))) => (unit + N (P (E (A G))) i0)%type) i (inl tt))
+               (id (Y G)) in
+           let (j0, s2) :=
+             action H g0
+               (existT (fun i1 : I (P (E (A H))) => (unit + N (P (E (A H))) i1)%type) j (inr m))
+               (id (Y H)) in
+           match s2 with
+           | inl tt =>
+               existT
+                 (fun i1 : I (P (E (A G))) * I (P (E (A H))) =>
+                  (unit + (N (P (E (A G))) (fst i1) + N (P (E (A H))) (snd i1)))%type) 
+                 (i0, j0) (inl tt)
+           | inr m0 =>
+               existT
+                 (fun i1 : I (P (E (A G))) * I (P (E (A H))) =>
+                  (unit + (N (P (E (A G))) (fst i1) + N (P (E (A H))) (snd i1)))%type) 
+                 (i0, j0) (inr (inr m0))
+           end
+       end) s)).
+{apply H1. rewrite Heqs. apply leq_tensor_left with (i:=i) (j:=i0) (m:=n0) (m':=n0). 
+apply reflexive. auto. auto. }
+rewrite Heqs in H2. simpl in H2. rewrite e3 in H2. rewrite e5 in H2. auto.
++ assert (exists k k1,
+action H g0
+       (existT (fun i : I (P (E (A H))) => (unit + N (P (E (A H))) i)%type) i0 (inr n0))
+       (id (Y H)) = 
+existT (fun i : I (P (E (A H))) => (unit + N (P (E (A H))) i)%type) k (inr k1)).
+{apply action_preserves_non_initial. }
+destruct H2. destruct H2. rewrite e4 in H2. inversion H2.
++ remember (existT
+          (fun i : I (P (E (A G))) * I (P (E (A H))) =>
+           (unit + (N (P (E (A G))) (fst i) + N (P (E (A H))) (snd i)))%type) 
+          (i, i0) (inr (inr n0))).
+assert 
+(s =
+     (let (x, s) := s in
+      (let
+         (i, j) as x0
+          return
+            (unit + (N (P (E (A G))) (fst x0) + N (P (E (A H))) (snd x0)) ->
+             M (partial_order_tensor (P (E (A G))) (P (E (A H))))) := x in
+       fun s0 : unit + (N (P (E (A G))) i + N (P (E (A H))) j) =>
+       match s0 with
+       | inl tt =>
+           let (i0, _) :=
+             action G g
+               (existT (fun i0 : I (P (E (A G))) => (unit + N (P (E (A G))) i0)%type) i
+                  (inl tt)) (id (Y G)) in
+           let (j0, _) :=
+             action H g0
+               (existT (fun i1 : I (P (E (A H))) => (unit + N (P (E (A H))) i1)%type) j
+                  (inl tt)) (id (Y H)) in
+           existT
+             (fun i1 : I (P (E (A G))) * I (P (E (A H))) =>
+              (unit + (N (P (E (A G))) (fst i1) + N (P (E (A H))) (snd i1)))%type) 
+             (i0, j0) (inl tt)
+       | inr (inl m) =>
+           let (i0, s1) :=
+             action G g
+               (existT (fun i0 : I (P (E (A G))) => (unit + N (P (E (A G))) i0)%type) i
+                  (inr m)) (id (Y G)) in
+           match s1 with
+           | inl tt =>
+               let (j0, _) :=
+                 action H g0
+                   (existT (fun i1 : I (P (E (A H))) => (unit + N (P (E (A H))) i1)%type) j
+                      (inl tt)) (id (Y H)) in
+               existT
+                 (fun i1 : I (P (E (A G))) * I (P (E (A H))) =>
+                  (unit + (N (P (E (A G))) (fst i1) + N (P (E (A H))) (snd i1)))%type)
+                 (i0, j0) (inl tt)
+           | inr m0 =>
+               let (j0, _) :=
+                 action H g0
+                   (existT (fun i1 : I (P (E (A H))) => (unit + N (P (E (A H))) i1)%type) j
+                      (inl tt)) (id (Y H)) in
+               existT
+                 (fun i1 : I (P (E (A G))) * I (P (E (A H))) =>
+                  (unit + (N (P (E (A G))) (fst i1) + N (P (E (A H))) (snd i1)))%type)
+                 (i0, j0) (inr (inl m0))
+           end
+       | inr (inr m) =>
+           let (i0, _) :=
+             action G g
+               (existT (fun i0 : I (P (E (A G))) => (unit + N (P (E (A G))) i0)%type) i
+                  (inl tt)) (id (Y G)) in
+           let (j0, s2) :=
+             action H g0
+               (existT (fun i1 : I (P (E (A H))) => (unit + N (P (E (A H))) i1)%type) j
+                  (inr m)) (id (Y H)) in
+           match s2 with
+           | inl tt =>
+               existT
+                 (fun i1 : I (P (E (A G))) * I (P (E (A H))) =>
+                  (unit + (N (P (E (A G))) (fst i1) + N (P (E (A H))) (snd i1)))%type)
+                 (i0, j0) (inl tt)
+           | inr m0 =>
+               existT
+                 (fun i1 : I (P (E (A G))) * I (P (E (A H))) =>
+                  (unit + (N (P (E (A G))) (fst i1) + N (P (E (A H))) (snd i1)))%type)
+                 (i0, j0) (inr (inr m0))
+           end
+       end) s)).
+{apply H1. rewrite Heqs. apply leq_tensor_right with (i:=i) (j:=i0)
+(m:=n0) (m':=n0). apply reflexive. auto. auto. }
+rewrite Heqs in H2. rewrite e3 in H2. rewrite e4 in H2. auto.
+- intros. destruct h. flatten_all; subst; simpl in *; destruct H0.
++ remember (existT
+          (fun i : I (P (E (A G))) * I (P (E (A H))) =>
+           (unit + (N (P (E (A G))) (fst i) + N (P (E (A H))) (snd i)))%type)
+          (i, i0) (inl tt)).
+assert (s =
+     (let (x, s) := s in
+      (let
+         (i, j) as x0
+          return
+            (unit + (N (P (E (A G))) (fst x0) + N (P (E (A H))) (snd x0)) ->
+             M (partial_order_tensor (P (E (A G))) (P (E (A H))))) := x in
+       fun s0 : unit + (N (P (E (A G))) i + N (P (E (A H))) j) =>
+       match s0 with
+       | inl tt =>
+           let (i0, _) :=
+             action G (id (X G))
+               (existT
+                  (fun i0 : I (P (E (A G))) => (unit + N (P (E (A G))) i0)%type) i
+                  (inl tt)) g in
+           let (j0, _) :=
+             action H (id (X H))
+               (existT
+                  (fun i1 : I (P (E (A H))) => (unit + N (P (E (A H))) i1)%type) j
+                  (inl tt)) g0 in
+           existT
+             (fun i1 : I (P (E (A G))) * I (P (E (A H))) =>
+              (unit + (N (P (E (A G))) (fst i1) + N (P (E (A H))) (snd i1)))%type)
+             (i0, j0) (inl tt)
+       | inr (inl m) =>
+           let (i0, s1) :=
+             action G (id (X G))
+               (existT
+                  (fun i0 : I (P (E (A G))) => (unit + N (P (E (A G))) i0)%type) i
+                  (inr m)) g in
+           match s1 with
+           | inl tt =>
+               let (j0, _) :=
+                 action H (id (X H))
+                   (existT
+                      (fun i1 : I (P (E (A H))) => (unit + N (P (E (A H))) i1)%type)
+                      j (inl tt)) g0 in
+               existT
+                 (fun i1 : I (P (E (A G))) * I (P (E (A H))) =>
+                  (unit + (N (P (E (A G))) (fst i1) + N (P (E (A H))) (snd i1)))%type)
+                 (i0, j0) (inl tt)
+           | inr m0 =>
+               let (j0, _) :=
+                 action H (id (X H))
+                   (existT
+                      (fun i1 : I (P (E (A H))) => (unit + N (P (E (A H))) i1)%type)
+                      j (inl tt)) g0 in
+               existT
+                 (fun i1 : I (P (E (A G))) * I (P (E (A H))) =>
+                  (unit + (N (P (E (A G))) (fst i1) + N (P (E (A H))) (snd i1)))%type)
+                 (i0, j0) (inr (inl m0))
+           end
+       | inr (inr m) =>
+           let (i0, _) :=
+             action G (id (X G))
+               (existT
+                  (fun i0 : I (P (E (A G))) => (unit + N (P (E (A G))) i0)%type) i
+                  (inl tt)) g in
+           let (j0, s2) :=
+             action H (id (X H))
+               (existT
+                  (fun i1 : I (P (E (A H))) => (unit + N (P (E (A H))) i1)%type) j
+                  (inr m)) g0 in
+           match s2 with
+           | inl tt =>
+               existT
+                 (fun i1 : I (P (E (A G))) * I (P (E (A H))) =>
+                  (unit + (N (P (E (A G))) (fst i1) + N (P (E (A H))) (snd i1)))%type)
+                 (i0, j0) (inl tt)
+           | inr m0 =>
+               existT
+                 (fun i1 : I (P (E (A G))) * I (P (E (A H))) =>
+                  (unit + (N (P (E (A G))) (fst i1) + N (P (E (A H))) (snd i1)))%type)
+                 (i0, j0) (inr (inr m0))
+           end
+       end) s)).
+{apply H1. rewrite Heqs. apply leq_tensor_least. } rewrite Heqs in H2.
+rewrite e3 in H2. rewrite e4 in H2. auto.
++ assert (exists k k1,
+action G (id (X G))
+       (existT (fun i : I (P (E (A G))) => (unit + N (P (E (A G))) i)%type) i
+          (inr n0)) g = 
+     existT (fun i : I (P (E (A G))) => (unit + N (P (E (A G))) i)%type) k (inr k1)).
+{apply action_preserves_non_initial. }
+destruct H2. destruct H2. rewrite e3 in H2. inversion H2.
++ remember (existT
+          (fun i : I (P (E (A G))) * I (P (E (A H))) =>
+           (unit + (N (P (E (A G))) (fst i) + N (P (E (A H))) (snd i)))%type)
+          (i, i0) (inr (inl n0))).
+assert (s =
+     (let (x, s) := s in
+      (let
+         (i, j) as x0
+          return
+            (unit + (N (P (E (A G))) (fst x0) + N (P (E (A H))) (snd x0)) ->
+             M (partial_order_tensor (P (E (A G))) (P (E (A H))))) := x in
+       fun s0 : unit + (N (P (E (A G))) i + N (P (E (A H))) j) =>
+       match s0 with
+       | inl tt =>
+           let (i0, _) :=
+             action G (id (X G))
+               (existT
+                  (fun i0 : I (P (E (A G))) => (unit + N (P (E (A G))) i0)%type) i
+                  (inl tt)) g in
+           let (j0, _) :=
+             action H (id (X H))
+               (existT
+                  (fun i1 : I (P (E (A H))) => (unit + N (P (E (A H))) i1)%type) j
+                  (inl tt)) g0 in
+           existT
+             (fun i1 : I (P (E (A G))) * I (P (E (A H))) =>
+              (unit + (N (P (E (A G))) (fst i1) + N (P (E (A H))) (snd i1)))%type)
+             (i0, j0) (inl tt)
+       | inr (inl m) =>
+           let (i0, s1) :=
+             action G (id (X G))
+               (existT
+                  (fun i0 : I (P (E (A G))) => (unit + N (P (E (A G))) i0)%type) i
+                  (inr m)) g in
+           match s1 with
+           | inl tt =>
+               let (j0, _) :=
+                 action H (id (X H))
+                   (existT
+                      (fun i1 : I (P (E (A H))) => (unit + N (P (E (A H))) i1)%type)
+                      j (inl tt)) g0 in
+               existT
+                 (fun i1 : I (P (E (A G))) * I (P (E (A H))) =>
+                  (unit + (N (P (E (A G))) (fst i1) + N (P (E (A H))) (snd i1)))%type)
+                 (i0, j0) (inl tt)
+           | inr m0 =>
+               let (j0, _) :=
+                 action H (id (X H))
+                   (existT
+                      (fun i1 : I (P (E (A H))) => (unit + N (P (E (A H))) i1)%type)
+                      j (inl tt)) g0 in
+               existT
+                 (fun i1 : I (P (E (A G))) * I (P (E (A H))) =>
+                  (unit + (N (P (E (A G))) (fst i1) + N (P (E (A H))) (snd i1)))%type)
+                 (i0, j0) (inr (inl m0))
+           end
+       | inr (inr m) =>
+           let (i0, _) :=
+             action G (id (X G))
+               (existT
+                  (fun i0 : I (P (E (A G))) => (unit + N (P (E (A G))) i0)%type) i
+                  (inl tt)) g in
+           let (j0, s2) :=
+             action H (id (X H))
+               (existT
+                  (fun i1 : I (P (E (A H))) => (unit + N (P (E (A H))) i1)%type) j
+                  (inr m)) g0 in
+           match s2 with
+           | inl tt =>
+               existT
+                 (fun i1 : I (P (E (A G))) * I (P (E (A H))) =>
+                  (unit + (N (P (E (A G))) (fst i1) + N (P (E (A H))) (snd i1)))%type)
+                 (i0, j0) (inl tt)
+           | inr m0 =>
+               existT
+                 (fun i1 : I (P (E (A G))) * I (P (E (A H))) =>
+                  (unit + (N (P (E (A G))) (fst i1) + N (P (E (A H))) (snd i1)))%type)
+                 (i0, j0) (inr (inr m0))
+           end
+       end) s)).
+{apply H1. rewrite Heqs. apply leq_tensor_left with (i:=i) (j:=i0) (m:=n0) (m':=n0). 
+apply reflexive. auto. auto. }
+rewrite Heqs in H2. rewrite e3 in H2. rewrite e5 in H2. auto.
++ assert (exists k k1,
+action H (id (X H))
+       (existT (fun i : I (P (E (A H))) => (unit + N (P (E (A H))) i)%type) i0
+          (inr n0)) g0 = 
+     existT (fun i : I (P (E (A H))) => (unit + N (P (E (A H))) i)%type) k (inr k1)).
+{apply action_preserves_non_initial. }
+destruct H2. destruct H2. rewrite e4 in H2. inversion H2.
++ remember (existT
+          (fun i : I (P (E (A G))) * I (P (E (A H))) =>
+           (unit + (N (P (E (A G))) (fst i) + N (P (E (A H))) (snd i)))%type)
+          (i, i0) (inr (inr n0))).
+assert 
+(s =
+     (let (x, s) := s in
+      (let
+         (i, j) as x0
+          return
+            (unit + (N (P (E (A G))) (fst x0) + N (P (E (A H))) (snd x0)) ->
+             M (partial_order_tensor (P (E (A G))) (P (E (A H))))) := x in
+       fun s0 : unit + (N (P (E (A G))) i + N (P (E (A H))) j) =>
+       match s0 with
+       | inl tt =>
+           let (i0, _) :=
+             action G (id (X G))
+               (existT
+                  (fun i0 : I (P (E (A G))) => (unit + N (P (E (A G))) i0)%type) i
+                  (inl tt)) g in
+           let (j0, _) :=
+             action H (id (X H))
+               (existT
+                  (fun i1 : I (P (E (A H))) => (unit + N (P (E (A H))) i1)%type) j
+                  (inl tt)) g0 in
+           existT
+             (fun i1 : I (P (E (A G))) * I (P (E (A H))) =>
+              (unit + (N (P (E (A G))) (fst i1) + N (P (E (A H))) (snd i1)))%type)
+             (i0, j0) (inl tt)
+       | inr (inl m) =>
+           let (i0, s1) :=
+             action G (id (X G))
+               (existT
+                  (fun i0 : I (P (E (A G))) => (unit + N (P (E (A G))) i0)%type) i
+                  (inr m)) g in
+           match s1 with
+           | inl tt =>
+               let (j0, _) :=
+                 action H (id (X H))
+                   (existT
+                      (fun i1 : I (P (E (A H))) => (unit + N (P (E (A H))) i1)%type)
+                      j (inl tt)) g0 in
+               existT
+                 (fun i1 : I (P (E (A G))) * I (P (E (A H))) =>
+                  (unit + (N (P (E (A G))) (fst i1) + N (P (E (A H))) (snd i1)))%type)
+                 (i0, j0) (inl tt)
+           | inr m0 =>
+               let (j0, _) :=
+                 action H (id (X H))
+                   (existT
+                      (fun i1 : I (P (E (A H))) => (unit + N (P (E (A H))) i1)%type)
+                      j (inl tt)) g0 in
+               existT
+                 (fun i1 : I (P (E (A G))) * I (P (E (A H))) =>
+                  (unit + (N (P (E (A G))) (fst i1) + N (P (E (A H))) (snd i1)))%type)
+                 (i0, j0) (inr (inl m0))
+           end
+       | inr (inr m) =>
+           let (i0, _) :=
+             action G (id (X G))
+               (existT
+                  (fun i0 : I (P (E (A G))) => (unit + N (P (E (A G))) i0)%type) i
+                  (inl tt)) g in
+           let (j0, s2) :=
+             action H (id (X H))
+               (existT
+                  (fun i1 : I (P (E (A H))) => (unit + N (P (E (A H))) i1)%type) j
+                  (inr m)) g0 in
+           match s2 with
+           | inl tt =>
+               existT
+                 (fun i1 : I (P (E (A G))) * I (P (E (A H))) =>
+                  (unit + (N (P (E (A G))) (fst i1) + N (P (E (A H))) (snd i1)))%type)
+                 (i0, j0) (inl tt)
+           | inr m0 =>
+               existT
+                 (fun i1 : I (P (E (A G))) * I (P (E (A H))) =>
+                  (unit + (N (P (E (A G))) (fst i1) + N (P (E (A H))) (snd i1)))%type)
+                 (i0, j0) (inr (inr m0))
+           end
+       end) s)).
+{apply H1. rewrite Heqs. apply leq_tensor_right with (i:=i) (j:=i0) (m:=n0) (m':=n0).
+apply reflexive. auto. auto. }
+rewrite Heqs in H2. rewrite e4 in H2. rewrite e3 in H2. auto.
+- intros. destruct i. destruct
+(action G (fst g)
+       (existT (fun i1 : I (P (E (A G))) => (unit + N (P (E (A G))) i1)%type) i
+          (inl tt)) (fst h)).
+destruct (action H (snd g)
+       (existT (fun i2 : I (P (E (A H))) => (unit + N (P (E (A H))) i2)%type) i0
+          (inl tt)) (snd h)). refine (ex_intro _ (x,x0) _). auto.
+- intros. destruct i. destruct m. 
++ destruct (action G (fst g)
+       (existT (fun i1 : I (P (E (A G))) => (unit + N (P (E (A G))) i1)%type) i
+          (inr n)) (fst h)) eqn:eqn1. destruct s.
+++ assert (exists k k1,
+action G (fst g)
+         (existT (fun i1 : I (P (E (A G))) => (unit + N (P (E (A G))) i1)%type) i
+            (inr n)) (fst h) =
+existT (fun i : I (P (E (A G))) => (unit + N (P (E (A G))) i)%type) k (inr k1)).
+{apply action_preserves_non_initial. }
+destruct H0. destruct H0. rewrite eqn1 in H0. inversion H0.
+++ destruct (action H (snd g)
+       (existT (fun i1 : I (P (E (A H))) => (unit + N (P (E (A H))) i1)%type) i0
+          (inl tt)) (snd h)) eqn:eqn2. refine (ex_intro _ (x,x0) _). refine (ex_intro _ (inl n0) _).
+auto.
++ destruct (action G (fst g)
+       (existT (fun i1 : I (P (E (A G))) => (unit + N (P (E (A G))) i1)%type) i
+          (inl tt)) (fst h)) eqn:eqn1. destruct s.
+++ destruct (action H (snd g)
+       (existT (fun i1 : I (P (E (A H))) => (unit + N (P (E (A H))) i1)%type) i0
+          (inr n)) (snd h)) eqn:eqn2. destruct s.
++++ assert (exists k k1,
+action H (snd g)
+         (existT (fun i1 : I (P (E (A H))) => (unit + N (P (E (A H))) i1)%type) i0
+            (inr n)) (snd h) =
+existT (fun i : I (P (E (A H))) => (unit + N (P (E (A H))) i)%type) k
+         (inr k1)).
+{apply action_preserves_non_initial. }
+destruct H0. destruct H0. rewrite eqn2 in H0. inversion H0.
++++ refine (ex_intro _ (x,x0) _). refine (ex_intro _ (inr n0) _). auto.
+++ assert (exists k,
+action G (fst g)
+         (existT (fun i1 : I (P (E (A G))) => (unit + N (P (E (A G))) i1)%type) i
+            (inl tt)) (fst h) = 
+existT (fun i : I (P (E (A G))) => (unit + N (P (E (A G))) i)%type) k
+         (inl tt)).
+{apply action_preserves_initial. }
+destruct H0. rewrite eqn1 in H0. inversion H0.
+Defined.
+
+Definition asynchronous_game_tensor_left (G H: AsynchronousGame) 
+(neg : (finite_payoff_position (A G)) nil = (1)%Z)
+(pos : (finite_payoff_position (A H)) nil = (-1)%Z) : AsynchronousGame :=
+asynchronous_game_tensor_positive
+(asynchronous_game_lifting G neg 0)
+H
+(positive_lifting_is_positive G neg 0)
+pos.
+
+Definition asynchronous_game_tensor_right (G H: AsynchronousGame) 
+(pos : (finite_payoff_position (A G)) nil = (-1)%Z)
+(neg : (finite_payoff_position (A H)) nil = (1)%Z) : AsynchronousGame :=
+asynchronous_game_tensor_positive
+G
+(asynchronous_game_lifting H neg 0)
+pos
+(positive_lifting_is_positive H neg 0).
+
+Definition asynchronous_game_tensor_negative (G H: AsynchronousGame) 
+(neg1 : (finite_payoff_position (A G)) nil = (1)%Z)
+(neg2 : (finite_payoff_position (A H)) nil = (1)%Z) : AsynchronousGame :=
+asynchronous_game_tensor_positive
+(asynchronous_game_lifting G neg1 0)
+(asynchronous_game_lifting H neg2 0)
+(positive_lifting_is_positive G neg1 0)
+(positive_lifting_is_positive H neg2 0).
+
+Definition asynchronous_game_tensor (G H: AsynchronousGame) :
+AsynchronousGame :=
+match initial_payoff (A G), initial_payoff (A H) with
+| left p, left p' => asynchronous_game_tensor_positive G H p p'
+| left p, right p' => asynchronous_game_tensor_right G H p p'
+| right p, left p' => asynchronous_game_tensor_left G H p p'
+| right p, right p' => asynchronous_game_tensor_negative G H p p'
+end.
+
